<?xml version="1.0"?>
<rdf:RDF xmlns="https://w3id.org/metpo/metpo.owl#"
     xml:base="https://w3id.org/metpo/metpo.owl"
     xmlns:dce="http://purl.org/dc/elements/1.1/"
     xmlns:obo="http://purl.obolibrary.org/obo/"
     xmlns:owl="http://www.w3.org/2002/07/owl#"
     xmlns:rdf="http://www.w3.org/1999/02/22-rdf-syntax-ns#"
     xmlns:xml="http://www.w3.org/XML/1998/namespace"
     xmlns:xsd="http://www.w3.org/2001/XMLSchema#"
     xmlns:rdfs="http://www.w3.org/2000/01/rdf-schema#"
     xmlns:metpo="https://w3id.org/metpo/"
     xmlns:dcterms="http://purl.org/dc/terms/"
     xmlns:oboInOwl="http://www.geneontology.org/formats/oboInOwl#">
    <owl:Ontology rdf:about="https://w3id.org/metpo/metpo.owl">
        <owl:versionIRI rdf:resource="https://w3id.org/metpo/metpo/releases/2025-03-13/metpo.owl"/>
        <dcterms:description>None</dcterms:description>
        <dcterms:license rdf:resource="https://creativecommons.org/licenses/unspecified"/>
        <dcterms:title>METPO</dcterms:title>
        <owl:versionInfo>2025-03-13</owl:versionInfo>
    </owl:Ontology>
    


    <!-- 
    ///////////////////////////////////////////////////////////////////////////////////////
    //
    // Annotation properties
    //
    ///////////////////////////////////////////////////////////////////////////////////////
     -->

    


    <!-- http://purl.obolibrary.org/obo/IAO_0000115 -->

    <owl:AnnotationProperty rdf:about="http://purl.obolibrary.org/obo/IAO_0000115"/>
    


    <!-- http://purl.org/dc/terms/description -->

    <owl:AnnotationProperty rdf:about="http://purl.org/dc/terms/description">
        <rdfs:label>description</rdfs:label>
    </owl:AnnotationProperty>
    


    <!-- http://purl.org/dc/terms/license -->

    <owl:AnnotationProperty rdf:about="http://purl.org/dc/terms/license">
        <rdfs:label>license</rdfs:label>
    </owl:AnnotationProperty>
    


    <!-- http://purl.org/dc/terms/title -->

    <owl:AnnotationProperty rdf:about="http://purl.org/dc/terms/title">
        <rdfs:label>title</rdfs:label>
    </owl:AnnotationProperty>
    


    <!-- http://www.geneontology.org/formats/oboInOwl#hasExactSynonym -->

    <owl:AnnotationProperty rdf:about="http://www.geneontology.org/formats/oboInOwl#hasExactSynonym"/>
    


    <!-- https://w3id.org/metpo/BactoTrait -->

    <owl:AnnotationProperty rdf:about="https://w3id.org/metpo/BactoTrait"/>
    


    <!-- 
    ///////////////////////////////////////////////////////////////////////////////////////
    //
    // Classes
    //
    ///////////////////////////////////////////////////////////////////////////////////////
     -->

    


    <!-- https://w3id.org/metpo/GenomicFeature -->

    <owl:Class rdf:about="https://w3id.org/metpo/GenomicFeature"/>
    


    <!-- https://w3id.org/metpo/NamedThing -->

    <owl:Class rdf:about="https://w3id.org/metpo/NamedThing"/>
    


    <!-- https://w3id.org/metpo/000001 -->

    <owl:Class rdf:about="https://w3id.org/metpo/000001">
        <rdfs:subClassOf rdf:resource="https://w3id.org/metpo/NamedThing"/>
        <rdfs:label>Temperature</rdfs:label>
    </owl:Class>
    


    <!-- https://w3id.org/metpo/000002 -->

    <owl:Class rdf:about="https://w3id.org/metpo/000002">
        <rdfs:subClassOf rdf:resource="https://w3id.org/metpo/NamedThing"/>
        <rdfs:label>Salinity</rdfs:label>
    </owl:Class>
    


    <!-- https://w3id.org/metpo/000003 -->

    <owl:Class rdf:about="https://w3id.org/metpo/000003">
        <rdfs:subClassOf rdf:resource="https://w3id.org/metpo/NamedThing"/>
        <rdfs:label>pH</rdfs:label>
    </owl:Class>
    


    <!-- https://w3id.org/metpo/000004 -->

    <owl:Class rdf:about="https://w3id.org/metpo/000004">
        <rdfs:subClassOf rdf:resource="https://w3id.org/metpo/NamedThing"/>
        <rdfs:label>Oxygen</rdfs:label>
    </owl:Class>
    


    <!-- https://w3id.org/metpo/000005 -->

    <owl:Class rdf:about="https://w3id.org/metpo/000005">
        <rdfs:subClassOf rdf:resource="https://w3id.org/metpo/NamedThing"/>
        <rdfs:label>Trophic type</rdfs:label>
    </owl:Class>
    


    <!-- https://w3id.org/metpo/000006 -->

    <owl:Class rdf:about="https://w3id.org/metpo/000006">
        <rdfs:subClassOf rdf:resource="https://w3id.org/metpo/NamedThing"/>
        <rdfs:label>Motility</rdfs:label>
    </owl:Class>
    


    <!-- https://w3id.org/metpo/000007 -->

    <owl:Class rdf:about="https://w3id.org/metpo/000007">
        <rdfs:subClassOf rdf:resource="https://w3id.org/metpo/NamedThing"/>
        <rdfs:label>Sporulation</rdfs:label>
    </owl:Class>
    


    <!-- https://w3id.org/metpo/000008 -->

    <owl:Class rdf:about="https://w3id.org/metpo/000008">
        <rdfs:subClassOf rdf:resource="https://w3id.org/metpo/NamedThing"/>
        <rdfs:label>Pressure</rdfs:label>
    </owl:Class>
    


    <!-- https://w3id.org/metpo/000009 -->

    <owl:Class rdf:about="https://w3id.org/metpo/000009">
        <rdfs:subClassOf rdf:resource="https://w3id.org/metpo/GenomicFeature"/>
        <rdfs:label>GC content</rdfs:label>
    </owl:Class>
    


    <!-- https://w3id.org/metpo/000010 -->

    <owl:Class rdf:about="https://w3id.org/metpo/000010">
        <rdfs:subClassOf rdf:resource="https://w3id.org/metpo/NamedThing"/>
        <rdfs:label>Cell Width</rdfs:label>
    </owl:Class>
    


    <!-- https://w3id.org/metpo/000011 -->

    <owl:Class rdf:about="https://w3id.org/metpo/000011">
        <rdfs:subClassOf rdf:resource="https://w3id.org/metpo/NamedThing"/>
        <rdfs:label>Cell Length</rdfs:label>
    </owl:Class>
    


    <!-- https://w3id.org/metpo/000012 -->

    <owl:Class rdf:about="https://w3id.org/metpo/000012">
        <rdfs:subClassOf rdf:resource="https://w3id.org/metpo/NamedThing"/>
        <rdfs:label>Temperature Optimum</rdfs:label>
    </owl:Class>
    


    <!-- https://w3id.org/metpo/000013 -->

    <owl:Class rdf:about="https://w3id.org/metpo/000013">
        <rdfs:subClassOf rdf:resource="https://w3id.org/metpo/NamedThing"/>
        <rdfs:label>Temperature Range</rdfs:label>
    </owl:Class>
    


    <!-- https://w3id.org/metpo/000014 -->

    <owl:Class rdf:about="https://w3id.org/metpo/000014">
        <rdfs:subClassOf rdf:resource="https://w3id.org/metpo/NamedThing"/>
        <rdfs:label>pH Optimum</rdfs:label>
    </owl:Class>
    


    <!-- https://w3id.org/metpo/000015 -->

    <owl:Class rdf:about="https://w3id.org/metpo/000015">
        <rdfs:subClassOf rdf:resource="https://w3id.org/metpo/NamedThing"/>
        <rdfs:label>pH Range</rdfs:label>
    </owl:Class>
    


    <!-- https://w3id.org/metpo/000016 -->

    <owl:Class rdf:about="https://w3id.org/metpo/000016">
        <rdfs:subClassOf rdf:resource="https://w3id.org/metpo/NamedThing"/>
        <rdfs:label>NaCl Optimum</rdfs:label>
    </owl:Class>
    


    <!-- https://w3id.org/metpo/000017 -->

    <owl:Class rdf:about="https://w3id.org/metpo/000017">
        <rdfs:subClassOf rdf:resource="https://w3id.org/metpo/NamedThing"/>
        <rdfs:label>NaCl Range</rdfs:label>
    </owl:Class>
    


    <!-- https://w3id.org/metpo/000018 -->

    <owl:Class rdf:about="https://w3id.org/metpo/000018">
        <rdfs:subClassOf rdf:resource="https://w3id.org/metpo/NamedThing"/>
        <rdfs:label>pH delta</rdfs:label>
    </owl:Class>
    


    <!-- https://w3id.org/metpo/000019 -->

    <owl:Class rdf:about="https://w3id.org/metpo/000019">
        <rdfs:subClassOf rdf:resource="https://w3id.org/metpo/NamedThing"/>
        <rdfs:label>NaCl delta</rdfs:label>
    </owl:Class>
    


    <!-- https://w3id.org/metpo/000020 -->

    <owl:Class rdf:about="https://w3id.org/metpo/000020">
        <rdfs:subClassOf rdf:resource="https://w3id.org/metpo/NamedThing"/>
        <rdfs:label>Temperature Delta</rdfs:label>
    </owl:Class>
    


    <!-- https://w3id.org/metpo/000021 -->

    <owl:Class rdf:about="https://w3id.org/metpo/000021">
        <rdfs:subClassOf rdf:resource="https://w3id.org/metpo/NamedThing"/>
        <rdfs:label>Morphology</rdfs:label>
    </owl:Class>
    


    <!-- https://w3id.org/metpo/000022 -->

    <owl:Class rdf:about="https://w3id.org/metpo/000022">
        <rdfs:subClassOf rdf:resource="https://w3id.org/metpo/NamedThing"/>
        <rdfs:label>Other</rdfs:label>
    </owl:Class>
    


    <!-- https://w3id.org/metpo/000023 -->

    <owl:Class rdf:about="https://w3id.org/metpo/000023">
        <rdfs:subClassOf rdf:resource="https://w3id.org/metpo/000001"/>
        <obo:IAO_0000115>A microorganism that grows optimally at temperatures below 15°C and can grow at temperatures below 20°C.</obo:IAO_0000115>
        <rdfs:label>Psychrophile</rdfs:label>
    </owl:Class>
    


    <!-- https://w3id.org/metpo/000024 -->

    <owl:Class rdf:about="https://w3id.org/metpo/000024">
        <rdfs:subClassOf rdf:resource="https://w3id.org/metpo/000001"/>
        <obo:IAO_0000115>A microorganism that can grow at temperatures near 0°C but has optimal growth at higher temperatures.</obo:IAO_0000115>
        <rdfs:label>Psychrotolerant</rdfs:label>
    </owl:Class>
    


    <!-- https://w3id.org/metpo/000025 -->

    <owl:Class rdf:about="https://w3id.org/metpo/000025">
        <rdfs:subClassOf rdf:resource="https://w3id.org/metpo/000001"/>
        <obo:IAO_0000115>A microorganism that grows optimally at moderate temperatures, typically between 20°C and 45°C.</obo:IAO_0000115>
        <rdfs:label>Mesophilie</rdfs:label>
    </owl:Class>
    


    <!-- https://w3id.org/metpo/000026 -->

    <owl:Class rdf:about="https://w3id.org/metpo/000026">
        <rdfs:subClassOf rdf:resource="https://w3id.org/metpo/000001"/>
        <obo:IAO_0000115>A microorganism that can grow at temperatures near 50°C but has optimal growth at lower temperatures.</obo:IAO_0000115>
        <rdfs:label>Thermotolerant</rdfs:label>
    </owl:Class>
    


    <!-- https://w3id.org/metpo/000027 -->

    <owl:Class rdf:about="https://w3id.org/metpo/000027">
        <rdfs:subClassOf rdf:resource="https://w3id.org/metpo/000001"/>
        <obo:IAO_0000115>A microorganism that grows optimally at relatively high temperatures, typically between 45°C and 80°C.</obo:IAO_0000115>
        <rdfs:label>Thermophile</rdfs:label>
    </owl:Class>
    


    <!-- https://w3id.org/metpo/000028 -->

    <owl:Class rdf:about="https://w3id.org/metpo/000028">
        <rdfs:subClassOf rdf:resource="https://w3id.org/metpo/000001"/>
        <obo:IAO_0000115>A microorganism that grows optimally at temperatures between 60°C and 80°C.</obo:IAO_0000115>
        <rdfs:label>Extreme thermophile</rdfs:label>
    </owl:Class>
    


    <!-- https://w3id.org/metpo/000029 -->

    <owl:Class rdf:about="https://w3id.org/metpo/000029">
        <rdfs:subClassOf rdf:resource="https://w3id.org/metpo/000001"/>
        <obo:IAO_0000115>A microorganism that grows optimally at very high temperatures, above 80°C.</obo:IAO_0000115>
        <rdfs:label>Hyperthermophile</rdfs:label>
    </owl:Class>
    


    <!-- https://w3id.org/metpo/000030 -->

    <owl:Class rdf:about="https://w3id.org/metpo/000030">
        <rdfs:subClassOf rdf:resource="https://w3id.org/metpo/000001"/>
        <obo:IAO_0000115>A microorganism that grows optimally at temperatures above 90°C.</obo:IAO_0000115>
        <rdfs:label>Extreme hyperthermophile</rdfs:label>
    </owl:Class>
    


    <!-- https://w3id.org/metpo/000031 -->

    <owl:Class rdf:about="https://w3id.org/metpo/000031">
        <rdfs:subClassOf rdf:resource="https://w3id.org/metpo/000002"/>
        <obo:IAO_0000115>A microorganism that requires salt for optimal growth and survival.</obo:IAO_0000115>
        <oboInOwl:hasExactSynonym>Halophilic</oboInOwl:hasExactSynonym>
        <rdfs:label>Halophile</rdfs:label>
    </owl:Class>
    


    <!-- https://w3id.org/metpo/000032 -->

    <owl:Class rdf:about="https://w3id.org/metpo/000032">
        <rdfs:subClassOf rdf:resource="https://w3id.org/metpo/000002"/>
        <obo:IAO_0000115>A microorganism that does not require salt for optimal growth and survival.</obo:IAO_0000115>
        <oboInOwl:hasExactSynonym>Non-halophilic</oboInOwl:hasExactSynonym>
        <oboInOwl:hasExactSynonym>Nonhalophile</oboInOwl:hasExactSynonym>
        <rdfs:label>Non-halophile</rdfs:label>
    </owl:Class>
    


    <!-- https://w3id.org/metpo/000033 -->

    <owl:Class rdf:about="https://w3id.org/metpo/000033">
        <rdfs:subClassOf rdf:resource="https://w3id.org/metpo/000002"/>
        <obo:IAO_0000115>A microorganism that grows optimally in environments with low salt concentrations, typically between 2-5% NaCl.</obo:IAO_0000115>
        <oboInOwl:hasExactSynonym>Slightly halophilic</oboInOwl:hasExactSynonym>
        <rdfs:label>Slight halophile</rdfs:label>
    </owl:Class>
    


    <!-- https://w3id.org/metpo/000034 -->

    <owl:Class rdf:about="https://w3id.org/metpo/000034">
        <rdfs:subClassOf rdf:resource="https://w3id.org/metpo/000002"/>
        <obo:IAO_0000115>A microorganism that grows optimally in environments with moderate salt concentrations, typically between 5-20% NaCl.</obo:IAO_0000115>
        <oboInOwl:hasExactSynonym>Moderately halophilic</oboInOwl:hasExactSynonym>
        <rdfs:label>Moderate halophile</rdfs:label>
    </owl:Class>
    


    <!-- https://w3id.org/metpo/000035 -->

    <owl:Class rdf:about="https://w3id.org/metpo/000035">
        <rdfs:subClassOf rdf:resource="https://w3id.org/metpo/000002"/>
        <obo:IAO_0000115>A microorganism that grows optimally in environments with high salt concentrations, typically above 20% NaCl.</obo:IAO_0000115>
        <oboInOwl:hasExactSynonym>Extremely halophilic</oboInOwl:hasExactSynonym>
        <rdfs:label>Extreme halophile</rdfs:label>
    </owl:Class>
    


    <!-- https://w3id.org/metpo/000036 -->

    <owl:Class rdf:about="https://w3id.org/metpo/000036">
        <rdfs:subClassOf rdf:resource="https://w3id.org/metpo/000002"/>
        <obo:IAO_0000115>A microorganism that grows optimally in environments with both high salt concentrations and high pH (alkaline conditions).</obo:IAO_0000115>
        <rdfs:label>Halotolerant</rdfs:label>
    </owl:Class>
    


    <!-- https://w3id.org/metpo/000037 -->

    <owl:Class rdf:about="https://w3id.org/metpo/000037">
        <rdfs:subClassOf rdf:resource="https://w3id.org/metpo/000002"/>
        <obo:IAO_0000115>A microorganism that grows optimally in environments with both high salt concentrations (typically 2-5% NaCl, but can tolerate up to 25% NaCl) and high pH (typically 9-11, but can grow at pH values up to 12).</obo:IAO_0000115>
        <rdfs:label>Haloalkaliphile</rdfs:label>
    </owl:Class>
    


    <!-- https://w3id.org/metpo/000038 -->

    <owl:Class rdf:about="https://w3id.org/metpo/000038">
        <rdfs:subClassOf rdf:resource="https://w3id.org/metpo/000003"/>
        <obo:IAO_0000115>A microorganism that grows optimally at very low pH values, typically between pH 1 and 3.</obo:IAO_0000115>
        <oboInOwl:hasExactSynonym>Extreme acidophilic</oboInOwl:hasExactSynonym>
        <rdfs:label>Extreme Acidophile</rdfs:label>
    </owl:Class>
    


    <!-- https://w3id.org/metpo/000039 -->

    <owl:Class rdf:about="https://w3id.org/metpo/000039">
        <rdfs:subClassOf rdf:resource="https://w3id.org/metpo/000003"/>
        <obo:IAO_0000115>A microorganism that grows optimally at low pH values, typically below pH 5.</obo:IAO_0000115>
        <oboInOwl:hasExactSynonym>Acidophilic</oboInOwl:hasExactSynonym>
        <rdfs:label>Acidophile</rdfs:label>
    </owl:Class>
    


    <!-- https://w3id.org/metpo/000040 -->

    <owl:Class rdf:about="https://w3id.org/metpo/000040">
        <rdfs:subClassOf rdf:resource="https://w3id.org/metpo/000003"/>
        <obo:IAO_0000115>A microorganism that grows optimally at neutral pH values, typically around pH 7.</obo:IAO_0000115>
        <oboInOwl:hasExactSynonym>Neutrophilic</oboInOwl:hasExactSynonym>
        <rdfs:label>Neutrophile</rdfs:label>
    </owl:Class>
    


    <!-- https://w3id.org/metpo/000041 -->

    <owl:Class rdf:about="https://w3id.org/metpo/000041">
        <rdfs:subClassOf rdf:resource="https://w3id.org/metpo/000003"/>
        <obo:IAO_0000115>A microorganism that grows optimally at high pH values, typically above pH 9.</obo:IAO_0000115>
        <rdfs:label>Alkaliphile</rdfs:label>
    </owl:Class>
    


    <!-- https://w3id.org/metpo/000042 -->

    <owl:Class rdf:about="https://w3id.org/metpo/000042">
        <rdfs:subClassOf rdf:resource="https://w3id.org/metpo/000003"/>
        <obo:IAO_0000115>A microorganism that can grow in acidic conditions below pH 5 but does not require them for optimal growth.</obo:IAO_0000115>
        <oboInOwl:hasExactSynonym>Alkaliphilic</oboInOwl:hasExactSynonym>
        <rdfs:label>Acid Tolerant</rdfs:label>
    </owl:Class>
    


    <!-- https://w3id.org/metpo/000043 -->

    <owl:Class rdf:about="https://w3id.org/metpo/000043">
        <rdfs:subClassOf rdf:resource="https://w3id.org/metpo/000003"/>
        <obo:IAO_0000115>A microorganism that can grow in alkaline conditions above pH 9 but does not require them for optimal growth.</obo:IAO_0000115>
        <oboInOwl:hasExactSynonym>Acid-tolerant</oboInOwl:hasExactSynonym>
        <rdfs:label>Alkali Tolerant</rdfs:label>
    </owl:Class>
    


    <!-- https://w3id.org/metpo/000044 -->

    <owl:Class rdf:about="https://w3id.org/metpo/000044">
        <rdfs:subClassOf rdf:resource="https://w3id.org/metpo/000003"/>
        <obo:IAO_0000115>A microorganism that grows optimally at very high pH values, typically above pH 10.</obo:IAO_0000115>
        <oboInOwl:hasExactSynonym>Alkali-tolerant</oboInOwl:hasExactSynonym>
        <rdfs:label>Extreme Alkaliphile</rdfs:label>
    </owl:Class>
    


    <!-- https://w3id.org/metpo/000045 -->

    <owl:Class rdf:about="https://w3id.org/metpo/000045">
        <rdfs:subClassOf rdf:resource="https://w3id.org/metpo/000003"/>
        <obo:IAO_0000115>A microorganism that can grow in acidic conditions but does not require them for optimal growth.</obo:IAO_0000115>
        <oboInOwl:hasExactSynonym>Extreme alkaliphilic</oboInOwl:hasExactSynonym>
        <rdfs:label>Facultative acidophile</rdfs:label>
    </owl:Class>
    


    <!-- https://w3id.org/metpo/000046 -->

    <owl:Class rdf:about="https://w3id.org/metpo/000046">
        <rdfs:subClassOf rdf:resource="https://w3id.org/metpo/000003"/>
        <obo:IAO_0000115>A microorganism that requires acidic conditions for growth and survival.</obo:IAO_0000115>
        <rdfs:label>Obligative acidophile</rdfs:label>
    </owl:Class>
    


    <!-- https://w3id.org/metpo/000047 -->

    <owl:Class rdf:about="https://w3id.org/metpo/000047">
        <rdfs:subClassOf rdf:resource="https://w3id.org/metpo/000004"/>
        <obo:IAO_0000115>A microorganism that requires oxygen for growth and metabolism.</obo:IAO_0000115>
        <oboInOwl:hasExactSynonym>Obligate aerobe</oboInOwl:hasExactSynonym>
        <oboInOwl:hasExactSynonym>Strict aerobe</oboInOwl:hasExactSynonym>
        <rdfs:label>Aerobe</rdfs:label>
    </owl:Class>
    


    <!-- https://w3id.org/metpo/000048 -->

    <owl:Class rdf:about="https://w3id.org/metpo/000048">
        <rdfs:subClassOf rdf:resource="https://w3id.org/metpo/000004"/>
        <obo:IAO_0000115>A microorganism that grows in the absence of oxygen and is unable to use oxygen for growth.</obo:IAO_0000115>
        <oboInOwl:hasExactSynonym>Obligate anaerobe</oboInOwl:hasExactSynonym>
        <oboInOwl:hasExactSynonym>Strict anaerobe</oboInOwl:hasExactSynonym>
        <rdfs:label>Anaerobe</rdfs:label>
    </owl:Class>
    


    <!-- https://w3id.org/metpo/000049 -->

    <owl:Class rdf:about="https://w3id.org/metpo/000049">
        <rdfs:subClassOf rdf:resource="https://w3id.org/metpo/000004"/>
        <obo:IAO_0000115>A microorganism that can grow with or without oxygen, using oxygen for respiration when available but capable of fermentation or anaerobic respiration in its absence.</obo:IAO_0000115>
        <oboInOwl:hasExactSynonym>Facultative aerobe</oboInOwl:hasExactSynonym>
        <rdfs:label>Facultative anaerobe</rdfs:label>
    </owl:Class>
    


    <!-- https://w3id.org/metpo/000050 -->

    <owl:Class rdf:about="https://w3id.org/metpo/000050">
        <rdfs:subClassOf rdf:resource="https://w3id.org/metpo/000004"/>
        <obo:IAO_0000115>A microorganism that primarily uses oxygen for respiration but can also grow without it using alternative metabolic pathways.</obo:IAO_0000115>
        <oboInOwl:hasExactSynonym>Facultative anaerobe</oboInOwl:hasExactSynonym>
        <rdfs:label>Facultative aerobe</rdfs:label>
    </owl:Class>
    


    <!-- https://w3id.org/metpo/000051 -->

    <owl:Class rdf:about="https://w3id.org/metpo/000051">
        <rdfs:subClassOf rdf:resource="https://w3id.org/metpo/000004"/>
        <obo:IAO_0000115>A microorganism that requires oxygen for growth but at concentrations lower than those found in air (typically 2-10% oxygen).</obo:IAO_0000115>
        <oboInOwl:hasExactSynonym>Microaerobe</oboInOwl:hasExactSynonym>
        <rdfs:label>Microaerophile</rdfs:label>
    </owl:Class>
    


    <!-- https://w3id.org/metpo/000052 -->

    <owl:Class rdf:about="https://w3id.org/metpo/000052">
        <rdfs:subClassOf rdf:resource="https://w3id.org/metpo/000004"/>
        <obo:IAO_0000115>A microorganism that does not use oxygen for growth but can survive and grow in its presence without being harmed.</obo:IAO_0000115>
        <oboInOwl:hasExactSynonym>Oxygen-tolerant</oboInOwl:hasExactSynonym>
        <rdfs:label>Aerotolerant</rdfs:label>
    </owl:Class>
    


    <!-- https://w3id.org/metpo/000053 -->

    <owl:Class rdf:about="https://w3id.org/metpo/000053">
        <rdfs:subClassOf rdf:resource="https://w3id.org/metpo/000004"/>
        <obo:IAO_0000115>A microorganism that can tolerate low levels of oxygen but does not require such conditions for growth.</obo:IAO_0000115>
        <oboInOwl:hasExactSynonym>Microoxic-tolerant</oboInOwl:hasExactSynonym>
        <rdfs:label>Microaerotolerant</rdfs:label>
    </owl:Class>
    


    <!-- https://w3id.org/metpo/000054 -->

    <owl:Class rdf:about="https://w3id.org/metpo/000054">
        <rdfs:subClassOf rdf:resource="https://w3id.org/metpo/000004"/>
        <obo:IAO_0000115>An anaerobic microorganism that does not use oxygen for metabolism but is not inhibited by its presence.</obo:IAO_0000115>
        <oboInOwl:hasExactSynonym>Oxygen-tolerant anaerobe</oboInOwl:hasExactSynonym>
        <rdfs:label>Aerotolerant anaerobe</rdfs:label>
    </owl:Class>
    


    <!-- https://w3id.org/metpo/000055 -->

    <owl:Class rdf:about="https://w3id.org/metpo/000055">
        <rdfs:subClassOf rdf:resource="https://w3id.org/metpo/000004"/>
        <obo:IAO_0000115>A microorganism that absolutely requires oxygen for growth and cannot grow under anaerobic conditions.</obo:IAO_0000115>
        <oboInOwl:hasExactSynonym>Aerobe</oboInOwl:hasExactSynonym>
        <oboInOwl:hasExactSynonym>Strict aerobe</oboInOwl:hasExactSynonym>
        <rdfs:label>Obligate aerobe</rdfs:label>
    </owl:Class>
    


    <!-- https://w3id.org/metpo/000056 -->

    <owl:Class rdf:about="https://w3id.org/metpo/000056">
        <rdfs:subClassOf rdf:resource="https://w3id.org/metpo/000004"/>
        <obo:IAO_0000115>A microorganism for which oxygen is toxic and inhibits growth, requiring strictly anaerobic conditions.</obo:IAO_0000115>
        <oboInOwl:hasExactSynonym>Anaerobe</oboInOwl:hasExactSynonym>
        <oboInOwl:hasExactSynonym>Strict anaerobe</oboInOwl:hasExactSynonym>
        <rdfs:label>Obligate anaerobe</rdfs:label>
    </owl:Class>
    


    <!-- https://w3id.org/metpo/000057 -->

    <owl:Class rdf:about="https://w3id.org/metpo/000057">
        <rdfs:subClassOf rdf:resource="https://w3id.org/metpo/000004"/>
        <obo:IAO_0000115>An organism that uses light energy for photosynthesis, producing oxygen as a byproduct.</obo:IAO_0000115>
        <oboInOwl:hasExactSynonym>Oxygenic phototrophic</oboInOwl:hasExactSynonym>
        <rdfs:label>Oxygenic phototroph</rdfs:label>
    </owl:Class>
    


    <!-- https://w3id.org/metpo/000058 -->

    <owl:Class rdf:about="https://w3id.org/metpo/000058">
        <rdfs:subClassOf rdf:resource="https://w3id.org/metpo/000004"/>
        <obo:IAO_0000115>An organism that uses light energy for photosynthesis without producing oxygen.</obo:IAO_0000115>
        <oboInOwl:hasExactSynonym>Anoxygenic phototrophic</oboInOwl:hasExactSynonym>
        <rdfs:label>Anoxygenic phototroph</rdfs:label>
    </owl:Class>
    


    <!-- https://w3id.org/metpo/000059 -->

    <owl:Class rdf:about="https://w3id.org/metpo/000059">
        <rdfs:subClassOf rdf:resource="https://w3id.org/metpo/000005"/>
        <obo:IAO_0000115>An organism that produces its own food from inorganic compounds.</obo:IAO_0000115>
        <oboInOwl:hasExactSynonym>Autotrophic</oboInOwl:hasExactSynonym>
        <rdfs:label>Autotroph</rdfs:label>
    </owl:Class>
    


    <!-- https://w3id.org/metpo/000060 -->

    <owl:Class rdf:about="https://w3id.org/metpo/000060">
        <rdfs:subClassOf rdf:resource="https://w3id.org/metpo/000005"/>
        <obo:IAO_0000115>An organism that uses light energy to fix carbon dioxide for growth.</obo:IAO_0000115>
        <oboInOwl:hasExactSynonym>Photoautotrophic</oboInOwl:hasExactSynonym>
        <rdfs:label>Photoautotroph</rdfs:label>
    </owl:Class>
    


    <!-- https://w3id.org/metpo/000061 -->

    <owl:Class rdf:about="https://w3id.org/metpo/000061">
        <rdfs:subClassOf rdf:resource="https://w3id.org/metpo/000005"/>
        <obo:IAO_0000115>An organism that uses energy from chemical reactions to fix carbon dioxide for growth.</obo:IAO_0000115>
        <oboInOwl:hasExactSynonym>Chemoautotrophic</oboInOwl:hasExactSynonym>
        <rdfs:label>Chemoautotroph</rdfs:label>
    </owl:Class>
    


    <!-- https://w3id.org/metpo/000062 -->

    <owl:Class rdf:about="https://w3id.org/metpo/000062">
        <rdfs:subClassOf rdf:resource="https://w3id.org/metpo/000005"/>
        <obo:IAO_0000115>An organism that obtains carbon from organic compounds.</obo:IAO_0000115>
        <oboInOwl:hasExactSynonym>Heterotrophic</oboInOwl:hasExactSynonym>
        <rdfs:label>Heterotroph</rdfs:label>
    </owl:Class>
    


    <!-- https://w3id.org/metpo/000063 -->

    <owl:Class rdf:about="https://w3id.org/metpo/000063">
        <rdfs:subClassOf rdf:resource="https://w3id.org/metpo/000005"/>
        <obo:IAO_0000115>An organism that uses light energy but obtains carbon from organic compounds.</obo:IAO_0000115>
        <oboInOwl:hasExactSynonym>Photoheterotrophic</oboInOwl:hasExactSynonym>
        <rdfs:label>Photoheterotroph</rdfs:label>
    </owl:Class>
    


    <!-- https://w3id.org/metpo/000064 -->

    <owl:Class rdf:about="https://w3id.org/metpo/000064">
        <rdfs:subClassOf rdf:resource="https://w3id.org/metpo/000005"/>
        <obo:IAO_0000115>An organism that obtains both energy and carbon from organic compounds.</obo:IAO_0000115>
        <oboInOwl:hasExactSynonym>Chemoheterotrophic</oboInOwl:hasExactSynonym>
        <rdfs:label>Chemoheterotroph</rdfs:label>
    </owl:Class>
    


    <!-- https://w3id.org/metpo/000065 -->

    <owl:Class rdf:about="https://w3id.org/metpo/000065">
        <rdfs:subClassOf rdf:resource="https://w3id.org/metpo/000005"/>
        <obo:IAO_0000115>An organism that obtains energy from the oxidation of inorganic compounds.</obo:IAO_0000115>
        <oboInOwl:hasExactSynonym>Lithotrophic</oboInOwl:hasExactSynonym>
        <rdfs:label>Lithotroph</rdfs:label>
    </owl:Class>
    


    <!-- https://w3id.org/metpo/000066 -->

    <owl:Class rdf:about="https://w3id.org/metpo/000066">
        <rdfs:subClassOf rdf:resource="https://w3id.org/metpo/000005"/>
        <obo:IAO_0000115>An organism that obtains energy from the oxidation of organic compounds.</obo:IAO_0000115>
        <oboInOwl:hasExactSynonym>Organotrophic</oboInOwl:hasExactSynonym>
        <rdfs:label>Organotroph</rdfs:label>
    </owl:Class>
    


    <!-- https://w3id.org/metpo/000067 -->

    <owl:Class rdf:about="https://w3id.org/metpo/000067">
        <rdfs:subClassOf rdf:resource="https://w3id.org/metpo/000005"/>
        <obo:IAO_0000115>An organism that uses light as its primary energy source.</obo:IAO_0000115>
        <oboInOwl:hasExactSynonym>Phototrophic</oboInOwl:hasExactSynonym>
        <rdfs:label>Phototroph</rdfs:label>
    </owl:Class>
    


    <!-- https://w3id.org/metpo/000068 -->

    <owl:Class rdf:about="https://w3id.org/metpo/000068">
        <rdfs:subClassOf rdf:resource="https://w3id.org/metpo/000005"/>
        <obo:IAO_0000115>An organism that obtains energy from chemical reactions.</obo:IAO_0000115>
        <oboInOwl:hasExactSynonym>Chemotrophic</oboInOwl:hasExactSynonym>
        <rdfs:label>Chemotroph</rdfs:label>
    </owl:Class>
    


    <!-- https://w3id.org/metpo/000069 -->

    <owl:Class rdf:about="https://w3id.org/metpo/000069">
        <rdfs:subClassOf rdf:resource="https://w3id.org/metpo/000005"/>
        <obo:IAO_0000115>An organism adapted to environments with low nutrient levels.</obo:IAO_0000115>
        <oboInOwl:hasExactSynonym>Oligotrophic</oboInOwl:hasExactSynonym>
        <rdfs:label>Oligotroph</rdfs:label>
    </owl:Class>
    


    <!-- https://w3id.org/metpo/000070 -->

    <owl:Class rdf:about="https://w3id.org/metpo/000070">
        <rdfs:subClassOf rdf:resource="https://w3id.org/metpo/000005"/>
        <obo:IAO_0000115>An organism adapted to environments with high nutrient levels.</obo:IAO_0000115>
        <oboInOwl:hasExactSynonym>Copiotrophic</oboInOwl:hasExactSynonym>
        <rdfs:label>Copiotroph</rdfs:label>
    </owl:Class>
    


    <!-- https://w3id.org/metpo/000071 -->

    <owl:Class rdf:about="https://w3id.org/metpo/000071">
        <rdfs:subClassOf rdf:resource="https://w3id.org/metpo/000005"/>
        <obo:IAO_0000115>An organism that uses inorganic compounds for both energy and carbon.</obo:IAO_0000115>
        <oboInOwl:hasExactSynonym>Lithoautotrophic</oboInOwl:hasExactSynonym>
        <rdfs:label>Lithoautotroph</rdfs:label>
    </owl:Class>
    


    <!-- https://w3id.org/metpo/000072 -->

    <owl:Class rdf:about="https://w3id.org/metpo/000072">
        <rdfs:subClassOf rdf:resource="https://w3id.org/metpo/000005"/>
        <obo:IAO_0000115>An organism capable of both autotrophic and heterotrophic nutrition.</obo:IAO_0000115>
        <oboInOwl:hasExactSynonym>Mixotrophic</oboInOwl:hasExactSynonym>
        <rdfs:label>Mixotroph</rdfs:label>
    </owl:Class>
    


    <!-- https://w3id.org/metpo/000073 -->

    <owl:Class rdf:about="https://w3id.org/metpo/000073">
        <rdfs:subClassOf rdf:resource="https://w3id.org/metpo/000005"/>
        <obo:IAO_0000115>An organism that uses inorganic compounds for energy but organic compounds for carbon.</obo:IAO_0000115>
        <oboInOwl:hasExactSynonym>Lithoheterotrophic</oboInOwl:hasExactSynonym>
        <rdfs:label>Lithoheterotroph</rdfs:label>
    </owl:Class>
    


    <!-- https://w3id.org/metpo/000074 -->

    <owl:Class rdf:about="https://w3id.org/metpo/000074">
        <rdfs:subClassOf rdf:resource="https://w3id.org/metpo/000005"/>
        <obo:IAO_0000115>An organism that uses organic compounds for both energy and carbon.</obo:IAO_0000115>
        <oboInOwl:hasExactSynonym>Chemoorganoheterotrophic</oboInOwl:hasExactSynonym>
        <rdfs:label>Chemoorganoheterotroph</rdfs:label>
    </owl:Class>
    


    <!-- https://w3id.org/metpo/000075 -->

    <owl:Class rdf:about="https://w3id.org/metpo/000075">
        <rdfs:subClassOf rdf:resource="https://w3id.org/metpo/000005"/>
        <obo:IAO_0000115>An organism that uses inorganic compounds for energy and CO2 for carbon.</obo:IAO_0000115>
        <oboInOwl:hasExactSynonym>Chemolithoautotrophic</oboInOwl:hasExactSynonym>
        <rdfs:label>Chemolithoautotroph</rdfs:label>
    </owl:Class>
    


    <!-- https://w3id.org/metpo/000076 -->

    <owl:Class rdf:about="https://w3id.org/metpo/000076">
        <rdfs:subClassOf rdf:resource="https://w3id.org/metpo/000005"/>
        <obo:IAO_0000115>An organism that can use one-carbon compounds as a source of energy and carbon.</obo:IAO_0000115>
        <oboInOwl:hasExactSynonym>Methylotrophic</oboInOwl:hasExactSynonym>
        <rdfs:label>Methylotroph</rdfs:label>
    </owl:Class>
    


    <!-- https://w3id.org/metpo/000077 -->

    <owl:Class rdf:about="https://w3id.org/metpo/000077">
        <rdfs:subClassOf rdf:resource="https://w3id.org/metpo/000005"/>
        <obo:IAO_0000115>An organism that uses methane as its sole source of carbon and energy.</obo:IAO_0000115>
        <oboInOwl:hasExactSynonym>Methanotrophic</oboInOwl:hasExactSynonym>
        <rdfs:label>Methanotroph</rdfs:label>
    </owl:Class>
    


    <!-- https://w3id.org/metpo/000078 -->

    <owl:Class rdf:about="https://w3id.org/metpo/000078">
        <rdfs:subClassOf rdf:resource="https://w3id.org/metpo/000005"/>
        <obo:IAO_0000115>An organism that can use carbon monoxide as its sole source of energy and carbon.</obo:IAO_0000115>
        <oboInOwl:hasExactSynonym>Carbohydrogenotroph</oboInOwl:hasExactSynonym>
        <oboInOwl:hasExactSynonym>Carboxydrophile</oboInOwl:hasExactSynonym>
        <rdfs:label>Carboxydotroph</rdfs:label>
    </owl:Class>
    


    <!-- https://w3id.org/metpo/000079 -->

    <owl:Class rdf:about="https://w3id.org/metpo/000079">
        <rdfs:subClassOf rdf:resource="https://w3id.org/metpo/000005"/>
        <obo:IAO_0000115>An organism that obtains energy from the oxidation of molecular hydrogen.</obo:IAO_0000115>
        <oboInOwl:hasExactSynonym>Hydrogenophile</oboInOwl:hasExactSynonym>
        <oboInOwl:hasExactSynonym>Hydrogenophilic</oboInOwl:hasExactSynonym>
        <rdfs:label>Hydrogenotroph</rdfs:label>
    </owl:Class>
    


    <!-- https://w3id.org/metpo/000080 -->

    <owl:Class rdf:about="https://w3id.org/metpo/000080">
        <rdfs:subClassOf rdf:resource="https://w3id.org/metpo/000005"/>
        <obo:IAO_0000115>An organism that oxidizes hydrogen for energy.</obo:IAO_0000115>
        <oboInOwl:hasExactSynonym>Hydrogen-oxidizing</oboInOwl:hasExactSynonym>
        <rdfs:label>Hydrogen oxidizer</rdfs:label>
    </owl:Class>
    


    <!-- https://w3id.org/metpo/000081 -->

    <owl:Class rdf:about="https://w3id.org/metpo/000081">
        <rdfs:subClassOf rdf:resource="https://w3id.org/metpo/000005"/>
        <obo:IAO_0000115>An organism that produces hydrogen as a byproduct of its metabolism.</obo:IAO_0000115>
        <oboInOwl:hasExactSynonym>Hydrogen-producing</oboInOwl:hasExactSynonym>
        <rdfs:label>Hydrogen producer</rdfs:label>
    </owl:Class>
    


    <!-- https://w3id.org/metpo/000082 -->

    <owl:Class rdf:about="https://w3id.org/metpo/000082">
        <rdfs:subClassOf rdf:resource="https://w3id.org/metpo/000005"/>
        <obo:IAO_0000115>An organism capable of converting atmospheric nitrogen into ammonia.</obo:IAO_0000115>
        <oboInOwl:hasExactSynonym>Nitrogen-fixing</oboInOwl:hasExactSynonym>
        <rdfs:label>Nitrogen fixer</rdfs:label>
    </owl:Class>
    


    <!-- https://w3id.org/metpo/000083 -->

    <owl:Class rdf:about="https://w3id.org/metpo/000083">
        <rdfs:subClassOf rdf:resource="https://w3id.org/metpo/000005"/>
        <obo:IAO_0000115>An organism that produces methane as a byproduct of its metabolism.</obo:IAO_0000115>
        <oboInOwl:hasExactSynonym>Methanogenic</oboInOwl:hasExactSynonym>
        <rdfs:label>Methanogen</rdfs:label>
    </owl:Class>
    


    <!-- https://w3id.org/metpo/000084 -->

    <owl:Class rdf:about="https://w3id.org/metpo/000084">
        <rdfs:subClassOf rdf:resource="https://w3id.org/metpo/000005"/>
        <obo:IAO_0000115>An organism that uses sulfate as an electron acceptor in anaerobic respiration.</obo:IAO_0000115>
        <oboInOwl:hasExactSynonym>Sulfate-reducing</oboInOwl:hasExactSynonym>
        <rdfs:label>Sulfate reducer</rdfs:label>
    </owl:Class>
    


    <!-- https://w3id.org/metpo/000085 -->

    <owl:Class rdf:about="https://w3id.org/metpo/000085">
        <rdfs:subClassOf rdf:resource="https://w3id.org/metpo/000005"/>
        <obo:IAO_0000115>An organism that oxidizes sulfur compounds for energy.</obo:IAO_0000115>
        <oboInOwl:hasExactSynonym>Sulfur-oxidizing</oboInOwl:hasExactSynonym>
        <rdfs:label>Sulfur oxidizer</rdfs:label>
    </owl:Class>
    


    <!-- https://w3id.org/metpo/000086 -->

    <owl:Class rdf:about="https://w3id.org/metpo/000086">
        <rdfs:subClassOf rdf:resource="https://w3id.org/metpo/000005"/>
        <obo:IAO_0000115>An organism that reduces nitrate to nitrogen gas in anaerobic respiration.</obo:IAO_0000115>
        <oboInOwl:hasExactSynonym>Denitrifying</oboInOwl:hasExactSynonym>
        <rdfs:label>Denitrifier</rdfs:label>
    </owl:Class>
    


    <!-- https://w3id.org/metpo/000087 -->

    <owl:Class rdf:about="https://w3id.org/metpo/000087">
        <rdfs:subClassOf rdf:resource="https://w3id.org/metpo/000005"/>
        <obo:IAO_0000115>An organism that requires or grows better in the presence of elevated levels of carbon dioxide.</obo:IAO_0000115>
        <oboInOwl:hasExactSynonym>Capnophilic</oboInOwl:hasExactSynonym>
        <rdfs:label>Capnophile</rdfs:label>
    </owl:Class>
    


    <!-- https://w3id.org/metpo/000088 -->

    <owl:Class rdf:about="https://w3id.org/metpo/000088">
        <rdfs:subClassOf rdf:resource="https://w3id.org/metpo/000006"/>
        <obo:IAO_0000115>A microorganism capable of self-propelled movement.</obo:IAO_0000115>
        <rdfs:label>Motile</rdfs:label>
    </owl:Class>
    


    <!-- https://w3id.org/metpo/000089 -->

    <owl:Class rdf:about="https://w3id.org/metpo/000089">
        <rdfs:subClassOf rdf:resource="https://w3id.org/metpo/000006"/>
        <obo:IAO_0000115>A microorganism incapable of self-propelled movement.</obo:IAO_0000115>
        <rdfs:label>Non-motile</rdfs:label>
    </owl:Class>
    


    <!-- https://w3id.org/metpo/000090 -->

    <owl:Class rdf:about="https://w3id.org/metpo/000090">
        <rdfs:subClassOf rdf:resource="https://w3id.org/metpo/000006"/>
        <obo:IAO_0000115>A motile microorganism that moves using one or more flagella.</obo:IAO_0000115>
        <rdfs:label>Flagellated</rdfs:label>
    </owl:Class>
    


    <!-- https://w3id.org/metpo/000091 -->

    <owl:Class rdf:about="https://w3id.org/metpo/000091">
        <rdfs:subClassOf rdf:resource="https://w3id.org/metpo/000006"/>
        <obo:IAO_0000115>A flagellated microorganism with flagella distributed over the entire cell surface.</obo:IAO_0000115>
        <rdfs:label>Peritrichous</rdfs:label>
    </owl:Class>
    


    <!-- https://w3id.org/metpo/000092 -->

    <owl:Class rdf:about="https://w3id.org/metpo/000092">
        <rdfs:subClassOf rdf:resource="https://w3id.org/metpo/000006"/>
        <obo:IAO_0000115>A flagellated microorganism with a tuft of flagella at one or both poles of the cell.</obo:IAO_0000115>
        <rdfs:label>Lophotrichous</rdfs:label>
    </owl:Class>
    


    <!-- https://w3id.org/metpo/000093 -->

    <owl:Class rdf:about="https://w3id.org/metpo/000093">
        <rdfs:subClassOf rdf:resource="https://w3id.org/metpo/000006"/>
        <obo:IAO_0000115>A flagellated microorganism with a single flagellum at one pole of the cell.</obo:IAO_0000115>
        <rdfs:label>Monotrichous</rdfs:label>
    </owl:Class>
    


    <!-- https://w3id.org/metpo/000094 -->

    <owl:Class rdf:about="https://w3id.org/metpo/000094">
        <rdfs:subClassOf rdf:resource="https://w3id.org/metpo/000006"/>
        <obo:IAO_0000115>A motile microorganism that moves using numerous short, hair-like structures called cilia.</obo:IAO_0000115>
        <rdfs:label>Ciliated</rdfs:label>
    </owl:Class>
    


    <!-- https://w3id.org/metpo/000095 -->

    <owl:Class rdf:about="https://w3id.org/metpo/000095">
        <rdfs:subClassOf rdf:resource="https://w3id.org/metpo/000006"/>
        <obo:IAO_0000115>A motile microorganism that moves by sliding over surfaces without the use of flagella or cilia.</obo:IAO_0000115>
        <rdfs:label>Gliding</rdfs:label>
    </owl:Class>
    


    <!-- https://w3id.org/metpo/000096 -->

    <owl:Class rdf:about="https://w3id.org/metpo/000096">
        <rdfs:subClassOf rdf:resource="https://w3id.org/metpo/000006"/>
        <obo:IAO_0000115>A motile microorganism that moves using type IV pili in a jerky, start-stop motion.</obo:IAO_0000115>
        <rdfs:label>Twitching</rdfs:label>
    </owl:Class>
    


    <!-- https://w3id.org/metpo/000097 -->

    <owl:Class rdf:about="https://w3id.org/metpo/000097">
        <rdfs:subClassOf rdf:resource="https://w3id.org/metpo/000006"/>
        <obo:IAO_0000115>A motile microorganism that moves passively over surfaces due to the production of extracellular substances.</obo:IAO_0000115>
        <rdfs:label>Sliding</rdfs:label>
    </owl:Class>
    


    <!-- https://w3id.org/metpo/000098 -->

    <owl:Class rdf:about="https://w3id.org/metpo/000098">
        <rdfs:subClassOf rdf:resource="https://w3id.org/metpo/000006"/>
        <obo:IAO_0000115>A motile microorganism capable of rapid, coordinated movement across surfaces in groups.</obo:IAO_0000115>
        <rdfs:label>Swarming</rdfs:label>
    </owl:Class>
    


    <!-- https://w3id.org/metpo/000099 -->

    <owl:Class rdf:about="https://w3id.org/metpo/000099">
        <rdfs:subClassOf rdf:resource="https://w3id.org/metpo/000007"/>
        <obo:IAO_0000115>A dormant, resistant structure formed within a bacterial cell.</obo:IAO_0000115>
        <rdfs:label>Endospores</rdfs:label>
    </owl:Class>
    


    <!-- https://w3id.org/metpo/000100 -->

    <owl:Class rdf:about="https://w3id.org/metpo/000100">
        <rdfs:subClassOf rdf:resource="https://w3id.org/metpo/000007"/>
        <obo:IAO_0000115>A spore formed outside the parent cell.</obo:IAO_0000115>
        <rdfs:label>Exospores</rdfs:label>
    </owl:Class>
    


    <!-- https://w3id.org/metpo/000101 -->

    <owl:Class rdf:about="https://w3id.org/metpo/000101">
        <rdfs:subClassOf rdf:resource="https://w3id.org/metpo/000007"/>
        <obo:IAO_0000115>A resting spore produced by myxobacteria during unfavorable conditions.</obo:IAO_0000115>
        <rdfs:label>Myxospores</rdfs:label>
    </owl:Class>
    


    <!-- https://w3id.org/metpo/000102 -->

    <owl:Class rdf:about="https://w3id.org/metpo/000102">
        <rdfs:subClassOf rdf:resource="https://w3id.org/metpo/000007"/>
        <obo:IAO_0000115>A type of spore formed by the fragmentation of fungal hyphae.</obo:IAO_0000115>
        <rdfs:label>Arthrospores</rdfs:label>
    </owl:Class>
    


    <!-- https://w3id.org/metpo/000103 -->

    <owl:Class rdf:about="https://w3id.org/metpo/000103">
        <rdfs:subClassOf rdf:resource="https://w3id.org/metpo/000007"/>
        <obo:IAO_0000115>Asexual spores produced by fungi, typically at the tips of specialized hyphae.</obo:IAO_0000115>
        <rdfs:label>Conidia</rdfs:label>
    </owl:Class>
    


    <!-- https://w3id.org/metpo/000104 -->

    <owl:Class rdf:about="https://w3id.org/metpo/000104">
        <rdfs:subClassOf rdf:resource="https://w3id.org/metpo/000007"/>
        <obo:IAO_0000115>Asexual spores produced within a sporangium.</obo:IAO_0000115>
        <rdfs:label>Sporangiospores</rdfs:label>
    </owl:Class>
    


    <!-- https://w3id.org/metpo/000105 -->

    <owl:Class rdf:about="https://w3id.org/metpo/000105">
        <rdfs:subClassOf rdf:resource="https://w3id.org/metpo/000007"/>
        <obo:IAO_0000115>A thick-walled resting spore resulting from the fusion of two compatible hyphae.</obo:IAO_0000115>
        <rdfs:label>Zygospores</rdfs:label>
    </owl:Class>
    


    <!-- https://w3id.org/metpo/000106 -->

    <owl:Class rdf:about="https://w3id.org/metpo/000106">
        <rdfs:subClassOf rdf:resource="https://w3id.org/metpo/000007"/>
        <obo:IAO_0000115>A large, thick-walled dormant cell formed by some cyanobacteria.</obo:IAO_0000115>
        <rdfs:label>Akinetes</rdfs:label>
    </owl:Class>
    


    <!-- https://w3id.org/metpo/000107 -->

    <owl:Class rdf:about="https://w3id.org/metpo/000107">
        <rdfs:subClassOf rdf:resource="https://w3id.org/metpo/000007"/>
        <obo:IAO_0000115>A thick-walled resting spore formed from a cell of a fungal hypha.</obo:IAO_0000115>
        <rdfs:label>Chlamydospores</rdfs:label>
    </owl:Class>
    


    <!-- https://w3id.org/metpo/000108 -->

    <owl:Class rdf:about="https://w3id.org/metpo/000108">
        <rdfs:subClassOf rdf:resource="https://w3id.org/metpo/000007"/>
        <obo:IAO_0000115>A protective cyst-like structure containing sporozoites in some protists.</obo:IAO_0000115>
        <rdfs:label>Sporocysts</rdfs:label>
    </owl:Class>
    


    <!-- https://w3id.org/metpo/000109 -->

    <owl:Class rdf:about="https://w3id.org/metpo/000109">
        <rdfs:subClassOf rdf:resource="https://w3id.org/metpo/000007"/>
        <obo:IAO_0000115>A dormant stage of some dinoflagellates, formed under unfavorable conditions.</obo:IAO_0000115>
        <rdfs:label>Hypnospores</rdfs:label>
    </owl:Class>
    


    <!-- https://w3id.org/metpo/000110 -->

    <owl:Class rdf:about="https://w3id.org/metpo/000110">
        <rdfs:subClassOf rdf:resource="https://w3id.org/metpo/000007"/>
        <obo:IAO_0000115>Small, multicellular propagules produced by some bryophytes for asexual reproduction.</obo:IAO_0000115>
        <rdfs:label>Gemmae</rdfs:label>
    </owl:Class>
    


    <!-- https://w3id.org/metpo/000111 -->

    <owl:Class rdf:about="https://w3id.org/metpo/000111">
        <rdfs:subClassOf rdf:resource="https://w3id.org/metpo/000007"/>
        <obo:IAO_0000115>A thick-walled sexual spore produced by oomycetes.</obo:IAO_0000115>
        <rdfs:label>Oospores</rdfs:label>
    </owl:Class>
    


    <!-- https://w3id.org/metpo/000112 -->

    <owl:Class rdf:about="https://w3id.org/metpo/000112">
        <rdfs:subClassOf rdf:resource="https://w3id.org/metpo/000007"/>
        <obo:IAO_0000115>A spore formed without fusion of gametes, typically in zygomycetes.</obo:IAO_0000115>
        <rdfs:label>Azygospores</rdfs:label>
    </owl:Class>
    


    <!-- https://w3id.org/metpo/000113 -->

    <owl:Class rdf:about="https://w3id.org/metpo/000113">
        <rdfs:subClassOf rdf:resource="https://w3id.org/metpo/000007"/>
        <obo:IAO_0000115>A resistant, dormant stage formed by some protists and bacteria.</obo:IAO_0000115>
        <rdfs:label>Cysts</rdfs:label>
    </owl:Class>
    


    <!-- https://w3id.org/metpo/000114 -->

    <owl:Class rdf:about="https://w3id.org/metpo/000114">
        <rdfs:subClassOf rdf:resource="https://w3id.org/metpo/000007"/>
        <obo:IAO_0000115>Sexual spores produced in an ascus, typically by ascomycete fungi.</obo:IAO_0000115>
        <rdfs:label>Ascospores</rdfs:label>
    </owl:Class>
    


    <!-- https://w3id.org/metpo/000115 -->

    <owl:Class rdf:about="https://w3id.org/metpo/000115">
        <rdfs:subClassOf rdf:resource="https://w3id.org/metpo/000007"/>
        <obo:IAO_0000115>Sexual spores produced on a basidium, typically by basidiomycete fungi.</obo:IAO_0000115>
        <rdfs:label>Basidiospores</rdfs:label>
    </owl:Class>
    


    <!-- https://w3id.org/metpo/000116 -->

    <owl:Class rdf:about="https://w3id.org/metpo/000116">
        <rdfs:subClassOf rdf:resource="https://w3id.org/metpo/000007"/>
        <obo:IAO_0000115>Asexual spores formed by the disarticulation of vegetative hyphae.</obo:IAO_0000115>
        <rdfs:label>Aleuriospores</rdfs:label>
    </owl:Class>
    


    <!-- https://w3id.org/metpo/000117 -->

    <owl:Class rdf:about="https://w3id.org/metpo/000117">
        <rdfs:subClassOf rdf:resource="https://w3id.org/metpo/000007"/>
        <obo:IAO_0000115>Asexual spores produced on a stalk-like structure called a sterigma.</obo:IAO_0000115>
        <rdfs:label>Stylospores</rdfs:label>
    </owl:Class>
    


    <!-- https://w3id.org/metpo/000118 -->

    <owl:Class rdf:about="https://w3id.org/metpo/000118">
        <rdfs:subClassOf rdf:resource="https://w3id.org/metpo/000007"/>
        <obo:IAO_0000115>A compact mass of hardened fungal mycelium containing food reserves.</obo:IAO_0000115>
        <rdfs:label>Sclerotia</rdfs:label>
    </owl:Class>
    


    <!-- https://w3id.org/metpo/000119 -->

    <owl:Class rdf:about="https://w3id.org/metpo/000119">
        <rdfs:subClassOf rdf:resource="https://w3id.org/metpo/000007"/>
        <obo:IAO_0000115>Motile spores with flagella, typically produced by algae and some fungi.</obo:IAO_0000115>
        <rdfs:label>Zoospores</rdfs:label>
    </owl:Class>
    


    <!-- https://w3id.org/metpo/000120 -->

    <owl:Class rdf:about="https://w3id.org/metpo/000120">
        <rdfs:subClassOf rdf:resource="https://w3id.org/metpo/000007"/>
        <obo:IAO_0000115>A type of resting spore produced by rust and smut fungi.</obo:IAO_0000115>
        <rdfs:label>Teliospores</rdfs:label>
    </owl:Class>
    


    <!-- https://w3id.org/metpo/000121 -->

    <owl:Class rdf:about="https://w3id.org/metpo/000121">
        <rdfs:subClassOf rdf:resource="https://w3id.org/metpo/000007"/>
        <obo:IAO_0000115>Asexual spores produced by rust fungi during their life cycle.</obo:IAO_0000115>
        <rdfs:label>Urediniospores</rdfs:label>
    </owl:Class>
    


    <!-- https://w3id.org/metpo/000122 -->

    <owl:Class rdf:about="https://w3id.org/metpo/000122">
        <rdfs:subClassOf rdf:resource="https://w3id.org/metpo/000007"/>
        <obo:IAO_0000115>Asexual spores produced within a pycnidium, a flask-shaped fruiting body.</obo:IAO_0000115>
        <rdfs:label>Pycnidiospores</rdfs:label>
    </owl:Class>
    


    <!-- https://w3id.org/metpo/000123 -->

    <owl:Class rdf:about="https://w3id.org/metpo/000123">
        <rdfs:subClassOf rdf:resource="https://w3id.org/metpo/000007"/>
        <obo:IAO_0000115>Asexual spores produced in chains at the tips of conidiophores.</obo:IAO_0000115>
        <rdfs:label>Acriospores</rdfs:label>
    </owl:Class>
    


    <!-- https://w3id.org/metpo/000124 -->

    <owl:Class rdf:about="https://w3id.org/metpo/000124">
        <rdfs:subClassOf rdf:resource="https://w3id.org/metpo/000007"/>
        <obo:IAO_0000115>Non-motile spores that lack flagella, typically produced by algae.</obo:IAO_0000115>
        <rdfs:label>Aplanospores</rdfs:label>
    </owl:Class>
    


    <!-- https://w3id.org/metpo/000125 -->

    <owl:Class rdf:about="https://w3id.org/metpo/000125">
        <rdfs:subClassOf rdf:resource="https://w3id.org/metpo/000007"/>
        <obo:IAO_0000115>Non-motile spores that lack the ability to swim.</obo:IAO_0000115>
        <rdfs:label>Statismospores</rdfs:label>
    </owl:Class>
    


    <!-- https://w3id.org/metpo/000126 -->

    <owl:Class rdf:about="https://w3id.org/metpo/000126">
        <rdfs:subClassOf rdf:resource="https://w3id.org/metpo/000008"/>
        <obo:IAO_0000115>An organism that can survive high pressure but does not require it for optimal growth.</obo:IAO_0000115>
        <rdfs:label>Barotolerant</rdfs:label>
    </owl:Class>
    


    <!-- https://w3id.org/metpo/000127 -->

    <owl:Class rdf:about="https://w3id.org/metpo/000127">
        <rdfs:subClassOf rdf:resource="https://w3id.org/metpo/000008"/>
        <obo:IAO_0000115>An organism that grows optimally under high pressure conditions.</obo:IAO_0000115>
        <oboInOwl:hasExactSynonym>Barophile</oboInOwl:hasExactSynonym>
        <oboInOwl:hasExactSynonym>Barophilic</oboInOwl:hasExactSynonym>
        <oboInOwl:hasExactSynonym>Piezophilic</oboInOwl:hasExactSynonym>
        <rdfs:label>Piezophile</rdfs:label>
    </owl:Class>
    


    <!-- https://w3id.org/metpo/000128 -->

    <owl:Class rdf:about="https://w3id.org/metpo/000128">
        <rdfs:subClassOf rdf:resource="https://w3id.org/metpo/000008"/>
        <obo:IAO_0000115>An organism that can tolerate high pressure but grows optimally at normal atmospheric pressure.</obo:IAO_0000115>
        <rdfs:label>Piezotolerant</rdfs:label>
    </owl:Class>
    


    <!-- https://w3id.org/metpo/000129 -->

    <owl:Class rdf:about="https://w3id.org/metpo/000129">
        <rdfs:subClassOf rdf:resource="https://w3id.org/metpo/000008"/>
        <obo:IAO_0000115>An organism that is adversely affected by high pressure conditions.</obo:IAO_0000115>
        <rdfs:label>Piezosensitive</rdfs:label>
    </owl:Class>
    


    <!-- https://w3id.org/metpo/000130 -->

    <owl:Class rdf:about="https://w3id.org/metpo/000130">
        <rdfs:subClassOf rdf:resource="https://w3id.org/metpo/000008"/>
        <obo:IAO_0000115>An organism that requires high pressure for growth and cannot grow at atmospheric pressure.</obo:IAO_0000115>
        <oboInOwl:hasExactSynonym>Obligate piezophile</oboInOwl:hasExactSynonym>
        <rdfs:label>Obligate barophile</rdfs:label>
    </owl:Class>
    


    <!-- https://w3id.org/metpo/000131 -->

    <owl:Class rdf:about="https://w3id.org/metpo/000131">
        <rdfs:subClassOf rdf:resource="https://w3id.org/metpo/000008"/>
        <obo:IAO_0000115>An organism that grows optimally under high pressure but can also grow at atmospheric pressure.</obo:IAO_0000115>
        <oboInOwl:hasExactSynonym>Facultative piezophile</oboInOwl:hasExactSynonym>
        <rdfs:label>Facultative barophile</rdfs:label>
    </owl:Class>
    


    <!-- https://w3id.org/metpo/000132 -->

    <owl:Class rdf:about="https://w3id.org/metpo/000132">
        <rdfs:subClassOf rdf:resource="https://w3id.org/metpo/000008"/>
        <obo:IAO_0000115>An organism adapted to extremely high pressure environments.</obo:IAO_0000115>
        <oboInOwl:hasExactSynonym>Hyperbarophilic</oboInOwl:hasExactSynonym>
        <rdfs:label>Hyperbarophile</rdfs:label>
    </owl:Class>
    


    <!-- https://w3id.org/metpo/000133 -->

    <owl:Class rdf:about="https://w3id.org/metpo/000133">
        <rdfs:subClassOf rdf:resource="https://w3id.org/metpo/000008"/>
        <obo:IAO_0000115>An organism adapted to low pressure environments.</obo:IAO_0000115>
        <oboInOwl:hasExactSynonym>Hypobarophilic</oboInOwl:hasExactSynonym>
        <rdfs:label>Hypobarophile</rdfs:label>
    </owl:Class>
    


    <!-- https://w3id.org/metpo/000134 -->

    <owl:Class rdf:about="https://w3id.org/metpo/000134">
        <rdfs:subClassOf rdf:resource="https://w3id.org/metpo/000008"/>
        <obo:IAO_0000115>An organism adapted to grow at standard atmospheric pressure.</obo:IAO_0000115>
        <rdfs:label>Atmospheric pressure-adapted</rdfs:label>
    </owl:Class>
    


    <!-- https://w3id.org/metpo/000135 -->

    <owl:Class rdf:about="https://w3id.org/metpo/000135">
        <rdfs:subClassOf rdf:resource="https://w3id.org/metpo/000008"/>
        <obo:IAO_0000115>An organism that grows optimally at moderately high pressures.</obo:IAO_0000115>
        <oboInOwl:hasExactSynonym>Moderate barophile</oboInOwl:hasExactSynonym>
        <rdfs:label>Moderate piezophile</rdfs:label>
    </owl:Class>
    


    <!-- https://w3id.org/metpo/000136 -->

    <owl:Class rdf:about="https://w3id.org/metpo/000136">
        <rdfs:subClassOf rdf:resource="https://w3id.org/metpo/000008"/>
        <obo:IAO_0000115>An organism that grows optimally at very high pressures.</obo:IAO_0000115>
        <oboInOwl:hasExactSynonym>Extreme barophile</oboInOwl:hasExactSynonym>
        <rdfs:label>Extreme piezophile</rdfs:label>
    </owl:Class>
    


    <!-- https://w3id.org/metpo/000137 -->

    <owl:Class rdf:about="https://w3id.org/metpo/000137">
        <rdfs:subClassOf rdf:resource="https://w3id.org/metpo/000008"/>
        <obo:IAO_0000115>An organism that can only grow within a narrow range of pressures.</obo:IAO_0000115>
        <oboInOwl:hasExactSynonym>Stenobaric</oboInOwl:hasExactSynonym>
        <rdfs:label>Stenopiezic</rdfs:label>
    </owl:Class>
    


    <!-- https://w3id.org/metpo/000138 -->

    <owl:Class rdf:about="https://w3id.org/metpo/000138">
        <rdfs:subClassOf rdf:resource="https://w3id.org/metpo/000008"/>
        <obo:IAO_0000115>An organism that can grow across a wide range of pressures.</obo:IAO_0000115>
        <oboInOwl:hasExactSynonym>Eurybaric</oboInOwl:hasExactSynonym>
        <rdfs:label>Eurypiezic</rdfs:label>
    </owl:Class>
    


    <!-- https://w3id.org/metpo/000139 -->

    <owl:Class rdf:about="https://w3id.org/metpo/000139">
        <rdfs:subClassOf rdf:resource="https://w3id.org/metpo/000008"/>
        <obo:IAO_0000115>An organism whose growth or metabolism is negatively affected by changes in pressure.</obo:IAO_0000115>
        <rdfs:label>Pressure-sensitive</rdfs:label>
    </owl:Class>
    


    <!-- https://w3id.org/metpo/000140 -->

    <owl:Class rdf:about="https://w3id.org/metpo/000140">
        <rdfs:subClassOf rdf:resource="https://w3id.org/metpo/000008"/>
        <obo:IAO_0000115>An organism that can withstand significant changes in pressure without adverse effects.</obo:IAO_0000115>
        <rdfs:label>Pressure-resistant</rdfs:label>
    </owl:Class>
    


    <!-- https://w3id.org/metpo/000141 -->

    <owl:Class rdf:about="https://w3id.org/metpo/000141">
        <rdfs:subClassOf rdf:resource="https://w3id.org/metpo/000008"/>
        <obo:IAO_0000115>An organism that has evolved to thrive under specific pressure conditions.</obo:IAO_0000115>
        <rdfs:label>Pressure-adapted</rdfs:label>
    </owl:Class>
    


    <!-- https://w3id.org/metpo/000142 -->

    <owl:Class rdf:about="https://w3id.org/metpo/000142">
        <rdfs:subClassOf rdf:resource="https://w3id.org/metpo/000008"/>
        <obo:IAO_0000115>An organism that grows optimally under both high pressure and acidic conditions.</obo:IAO_0000115>
        <oboInOwl:hasExactSynonym>Piezo-acidophilic</oboInOwl:hasExactSynonym>
        <rdfs:label>Piezo-acidophile</rdfs:label>
    </owl:Class>
    


    <!-- https://w3id.org/metpo/000143 -->

    <owl:Class rdf:about="https://w3id.org/metpo/000143">
        <rdfs:subClassOf rdf:resource="https://w3id.org/metpo/000008"/>
        <obo:IAO_0000115>An organism that grows optimally under both high pressure and alkaline conditions.</obo:IAO_0000115>
        <oboInOwl:hasExactSynonym>Piezo-alkaliphilic</oboInOwl:hasExactSynonym>
        <rdfs:label>Piezo-alkaliphile</rdfs:label>
    </owl:Class>
    


    <!-- https://w3id.org/metpo/000144 -->

    <owl:Class rdf:about="https://w3id.org/metpo/000144">
        <rdfs:subClassOf rdf:resource="https://w3id.org/metpo/000008"/>
        <obo:IAO_0000115>An organism that grows optimally under both high pressure and high salinity conditions.</obo:IAO_0000115>
        <oboInOwl:hasExactSynonym>Piezo-halophilic</oboInOwl:hasExactSynonym>
        <rdfs:label>Piezo-halophile</rdfs:label>
    </owl:Class>
    


    <!-- https://w3id.org/metpo/000145 -->

    <owl:Class rdf:about="https://w3id.org/metpo/000145">
        <rdfs:subClassOf rdf:resource="https://w3id.org/metpo/000008"/>
        <obo:IAO_0000115>An organism that grows optimally under both high pressure and low temperature conditions.</obo:IAO_0000115>
        <oboInOwl:hasExactSynonym>Piezo-psychrophilic</oboInOwl:hasExactSynonym>
        <rdfs:label>Piezo-psychrophile</rdfs:label>
    </owl:Class>
    


    <!-- https://w3id.org/metpo/000146 -->

    <owl:Class rdf:about="https://w3id.org/metpo/000146">
        <rdfs:subClassOf rdf:resource="https://w3id.org/metpo/000008"/>
        <obo:IAO_0000115>An organism that grows optimally under both high pressure and high temperature conditions.</obo:IAO_0000115>
        <oboInOwl:hasExactSynonym>Piezo-thermophilic</oboInOwl:hasExactSynonym>
        <rdfs:label>Piezo-thermophile</rdfs:label>
    </owl:Class>
    


    <!-- https://w3id.org/metpo/000147 -->

    <owl:Class rdf:about="https://w3id.org/metpo/000147">
        <rdfs:subClassOf rdf:resource="https://w3id.org/metpo/000008"/>
        <obo:IAO_0000115>An organism that uses inorganic compounds for energy and carbon under high pressure conditions.</obo:IAO_0000115>
        <oboInOwl:hasExactSynonym>Piezo-lithoautotrophic</oboInOwl:hasExactSynonym>
        <rdfs:label>Piezo-lithoautotrophe</rdfs:label>
    </owl:Class>
    


    <!-- https://w3id.org/metpo/000148 -->

    <owl:Class rdf:about="https://w3id.org/metpo/000148">
        <rdfs:subClassOf rdf:resource="https://w3id.org/metpo/000008"/>
        <obo:IAO_0000115>An organism that uses organic compounds for energy and carbon under high pressure conditions.</obo:IAO_0000115>
        <oboInOwl:hasExactSynonym>Piezo-chemoheterotrophic</oboInOwl:hasExactSynonym>
        <rdfs:label>Piezo-chemoheterotroph</rdfs:label>
    </owl:Class>
    


    <!-- https://w3id.org/metpo/000149 -->

    <owl:Class rdf:about="https://w3id.org/metpo/000149">
        <rdfs:subClassOf rdf:resource="https://w3id.org/metpo/000008"/>
        <obo:IAO_0000115>An organism adapted to low-nutrient environments under high pressure conditions.</obo:IAO_0000115>
        <oboInOwl:hasExactSynonym>Piezo-oligotrophic</oboInOwl:hasExactSynonym>
        <rdfs:label>Piezo-oligotroph</rdfs:label>
    </owl:Class>
    


    <!-- https://w3id.org/metpo/000150 -->

    <owl:Class rdf:about="https://w3id.org/metpo/000150">
        <rdfs:subClassOf rdf:resource="https://w3id.org/metpo/000008"/>
        <obo:IAO_0000115>An organism that lives within rock or mineral substrates under high pressure conditions.</obo:IAO_0000115>
        <rdfs:label>Piezo-endolithic</rdfs:label>
    </owl:Class>
    


    <!-- https://w3id.org/metpo/000151 -->

    <owl:Class rdf:about="https://w3id.org/metpo/000151">
        <rdfs:subClassOf rdf:resource="https://w3id.org/metpo/000008"/>
        <obo:IAO_0000115>An organism that can tolerate a range of pressure conditions but does not necessarily require high pressure for optimal growth.</obo:IAO_0000115>
        <rdfs:label>Piezo-tolerant</rdfs:label>
    </owl:Class>
    


    <!-- https://w3id.org/metpo/000152 -->

    <owl:Class rdf:about="https://w3id.org/metpo/000152">
        <rdfs:subClassOf rdf:resource="https://w3id.org/metpo/000009"/>
        <oboInOwl:hasExactSynonym>gc:low</oboInOwl:hasExactSynonym>
        <rdfs:label>GC% low ( &lt; 42.65)</rdfs:label>
        <metpo:BactoTrait>GC_&lt;=42.65</metpo:BactoTrait>
    </owl:Class>
    


    <!-- https://w3id.org/metpo/000153 -->

    <owl:Class rdf:about="https://w3id.org/metpo/000153">
        <rdfs:subClassOf rdf:resource="https://w3id.org/metpo/000009"/>
        <rdfs:label>GC% mid1 (42.65 - 57)</rdfs:label>
        <metpo:BactoTrait>GC_42.65_57.0</metpo:BactoTrait>
    </owl:Class>
    


    <!-- https://w3id.org/metpo/000154 -->

    <owl:Class rdf:about="https://w3id.org/metpo/000154">
        <rdfs:subClassOf rdf:resource="https://w3id.org/metpo/000009"/>
        <rdfs:label>GC% mid2 (57 - 66.3)</rdfs:label>
        <metpo:BactoTrait>GC_57.0_66.3</metpo:BactoTrait>
    </owl:Class>
    


    <!-- https://w3id.org/metpo/000155 -->

    <owl:Class rdf:about="https://w3id.org/metpo/000155">
        <rdfs:subClassOf rdf:resource="https://w3id.org/metpo/000009"/>
        <rdfs:label>GC% high ( &gt; 66.3)</rdfs:label>
        <metpo:BactoTrait>GC_&gt;66.3</metpo:BactoTrait>
    </owl:Class>
    


    <!-- https://w3id.org/metpo/000156 -->

    <owl:Class rdf:about="https://w3id.org/metpo/000156">
        <rdfs:subClassOf rdf:resource="https://w3id.org/metpo/000010"/>
        <rdfs:label>Cell width uM very low (&lt; 0.5)</rdfs:label>
        <metpo:BactoTrait>W_&lt;=0.5</metpo:BactoTrait>
    </owl:Class>
    


    <!-- https://w3id.org/metpo/000157 -->

    <owl:Class rdf:about="https://w3id.org/metpo/000157">
        <rdfs:subClassOf rdf:resource="https://w3id.org/metpo/000010"/>
        <rdfs:label>Cell width uM low (0.5 - 0.65)</rdfs:label>
        <metpo:BactoTrait>W_0.5_0.65</metpo:BactoTrait>
    </owl:Class>
    


    <!-- https://w3id.org/metpo/000158 -->

    <owl:Class rdf:about="https://w3id.org/metpo/000158">
        <rdfs:subClassOf rdf:resource="https://w3id.org/metpo/000010"/>
        <rdfs:label>Cell width uM mid (0.65 - 0.9)</rdfs:label>
        <metpo:BactoTrait>W_0.65_0.9</metpo:BactoTrait>
    </owl:Class>
    


    <!-- https://w3id.org/metpo/000159 -->

    <owl:Class rdf:about="https://w3id.org/metpo/000159">
        <rdfs:subClassOf rdf:resource="https://w3id.org/metpo/000010"/>
        <rdfs:label>Cell width uM high (&gt; 0.9)</rdfs:label>
        <metpo:BactoTrait>W_&gt;0.9</metpo:BactoTrait>
    </owl:Class>
    


    <!-- https://w3id.org/metpo/000160 -->

    <owl:Class rdf:about="https://w3id.org/metpo/000160">
        <rdfs:subClassOf rdf:resource="https://w3id.org/metpo/000011"/>
        <rdfs:label>Cell length uM very low (&lt;= 1.3)</rdfs:label>
        <metpo:BactoTrait>L_&lt;=1.3</metpo:BactoTrait>
    </owl:Class>
    


    <!-- https://w3id.org/metpo/000161 -->

    <owl:Class rdf:about="https://w3id.org/metpo/000161">
        <rdfs:subClassOf rdf:resource="https://w3id.org/metpo/000011"/>
        <rdfs:label>Cell length uM low (1.3 - 2)</rdfs:label>
        <metpo:BactoTrait>L_1.3_2</metpo:BactoTrait>
    </owl:Class>
    


    <!-- https://w3id.org/metpo/000162 -->

    <owl:Class rdf:about="https://w3id.org/metpo/000162">
        <rdfs:subClassOf rdf:resource="https://w3id.org/metpo/000011"/>
        <rdfs:label>Cell length uM mid (2 - 3)</rdfs:label>
        <metpo:BactoTrait>L_2_3</metpo:BactoTrait>
    </owl:Class>
    


    <!-- https://w3id.org/metpo/000163 -->

    <owl:Class rdf:about="https://w3id.org/metpo/000163">
        <rdfs:subClassOf rdf:resource="https://w3id.org/metpo/000011"/>
        <rdfs:label>Cell length uM high (&gt; 3)</rdfs:label>
        <metpo:BactoTrait>L_&gt;3</metpo:BactoTrait>
    </owl:Class>
    


    <!-- https://w3id.org/metpo/000164 -->

    <owl:Class rdf:about="https://w3id.org/metpo/000164">
        <rdfs:subClassOf rdf:resource="https://w3id.org/metpo/000012"/>
        <oboInOwl:hasExactSynonym>Psychrophile</oboInOwl:hasExactSynonym>
        <rdfs:label>Temperature Optimum C very low (&lt;= 10)</rdfs:label>
        <metpo:BactoTrait>TO_&lt;=10</metpo:BactoTrait>
    </owl:Class>
    


    <!-- https://w3id.org/metpo/000165 -->

    <owl:Class rdf:about="https://w3id.org/metpo/000165">
        <rdfs:subClassOf rdf:resource="https://w3id.org/metpo/000012"/>
        <oboInOwl:hasExactSynonym>Psychrophile</oboInOwl:hasExactSynonym>
        <oboInOwl:hasExactSynonym>Psychrotolerant</oboInOwl:hasExactSynonym>
        <rdfs:label>Temperature Optimum C low (10 - 22)</rdfs:label>
        <metpo:BactoTrait>TO_10_to_22</metpo:BactoTrait>
    </owl:Class>
    


    <!-- https://w3id.org/metpo/000166 -->

    <owl:Class rdf:about="https://w3id.org/metpo/000166">
        <rdfs:subClassOf rdf:resource="https://w3id.org/metpo/000012"/>
        <oboInOwl:hasExactSynonym>Mesophilie</oboInOwl:hasExactSynonym>
        <rdfs:label>Temperature Optimum C mid1 (22 - 27)</rdfs:label>
        <metpo:BactoTrait>TO_22_to_27</metpo:BactoTrait>
    </owl:Class>
    


    <!-- https://w3id.org/metpo/000167 -->

    <owl:Class rdf:about="https://w3id.org/metpo/000167">
        <rdfs:subClassOf rdf:resource="https://w3id.org/metpo/000012"/>
        <oboInOwl:hasExactSynonym>Mesophilie</oboInOwl:hasExactSynonym>
        <rdfs:label>Temperature Optimum C mid2 (27 - 30)</rdfs:label>
        <metpo:BactoTrait>TO_27_to_30</metpo:BactoTrait>
    </owl:Class>
    


    <!-- https://w3id.org/metpo/000168 -->

    <owl:Class rdf:about="https://w3id.org/metpo/000168">
        <rdfs:subClassOf rdf:resource="https://w3id.org/metpo/000012"/>
        <oboInOwl:hasExactSynonym>Mesophilie</oboInOwl:hasExactSynonym>
        <rdfs:label>Temperature Optimum C mid3 (30 - 34)</rdfs:label>
        <metpo:BactoTrait>TO_30_to_34</metpo:BactoTrait>
    </owl:Class>
    


    <!-- https://w3id.org/metpo/000169 -->

    <owl:Class rdf:about="https://w3id.org/metpo/000169">
        <rdfs:subClassOf rdf:resource="https://w3id.org/metpo/000012"/>
        <oboInOwl:hasExactSynonym>Mesophilie</oboInOwl:hasExactSynonym>
        <rdfs:label>Temperature Optimum C mid4 (34 - 40)</rdfs:label>
        <metpo:BactoTrait>TO_34_to_40</metpo:BactoTrait>
    </owl:Class>
    


    <!-- https://w3id.org/metpo/000170 -->

    <owl:Class rdf:about="https://w3id.org/metpo/000170">
        <rdfs:subClassOf rdf:resource="https://w3id.org/metpo/000012"/>
        <oboInOwl:hasExactSynonym>Thermophile</oboInOwl:hasExactSynonym>
        <rdfs:label>Temperature Optimum C high (&gt; 40)</rdfs:label>
        <metpo:BactoTrait>TO_&gt;40</metpo:BactoTrait>
    </owl:Class>
    


    <!-- https://w3id.org/metpo/000171 -->

    <owl:Class rdf:about="https://w3id.org/metpo/000171">
        <rdfs:subClassOf rdf:resource="https://w3id.org/metpo/000013"/>
        <oboInOwl:hasExactSynonym>Psychrophile</oboInOwl:hasExactSynonym>
        <rdfs:label>Temperature Range C very low (&lt;= 10)</rdfs:label>
        <metpo:BactoTrait>TR_&lt;=10</metpo:BactoTrait>
    </owl:Class>
    


    <!-- https://w3id.org/metpo/000172 -->

    <owl:Class rdf:about="https://w3id.org/metpo/000172">
        <rdfs:subClassOf rdf:resource="https://w3id.org/metpo/000013"/>
        <oboInOwl:hasExactSynonym>Psychrophile</oboInOwl:hasExactSynonym>
        <oboInOwl:hasExactSynonym>Psychrotolerant</oboInOwl:hasExactSynonym>
        <rdfs:label>Temperature Range C low (10 - 22)</rdfs:label>
        <metpo:BactoTrait>TR_10_to_22</metpo:BactoTrait>
    </owl:Class>
    


    <!-- https://w3id.org/metpo/000173 -->

    <owl:Class rdf:about="https://w3id.org/metpo/000173">
        <rdfs:subClassOf rdf:resource="https://w3id.org/metpo/000013"/>
        <oboInOwl:hasExactSynonym>Mesophilie</oboInOwl:hasExactSynonym>
        <rdfs:label>Temperature Range C mid1 (22 - 27)</rdfs:label>
        <metpo:BactoTrait>TR_22_to_27</metpo:BactoTrait>
    </owl:Class>
    


    <!-- https://w3id.org/metpo/000174 -->

    <owl:Class rdf:about="https://w3id.org/metpo/000174">
        <rdfs:subClassOf rdf:resource="https://w3id.org/metpo/000013"/>
        <oboInOwl:hasExactSynonym>Mesophilie</oboInOwl:hasExactSynonym>
        <rdfs:label>Temperature Range C mid2 (27 - 30)</rdfs:label>
        <metpo:BactoTrait>TR_27_to_30</metpo:BactoTrait>
    </owl:Class>
    


    <!-- https://w3id.org/metpo/000175 -->

    <owl:Class rdf:about="https://w3id.org/metpo/000175">
        <rdfs:subClassOf rdf:resource="https://w3id.org/metpo/000013"/>
        <oboInOwl:hasExactSynonym>Mesophilie</oboInOwl:hasExactSynonym>
        <rdfs:label>Temperature Range C mid3 (30 - 34)</rdfs:label>
        <metpo:BactoTrait>TR_30_to_34</metpo:BactoTrait>
    </owl:Class>
    


    <!-- https://w3id.org/metpo/000176 -->

    <owl:Class rdf:about="https://w3id.org/metpo/000176">
        <rdfs:subClassOf rdf:resource="https://w3id.org/metpo/000013"/>
        <oboInOwl:hasExactSynonym>Mesophilie</oboInOwl:hasExactSynonym>
        <rdfs:label>Temperature Range C mid4 (34 - 40)</rdfs:label>
        <metpo:BactoTrait>TR_34_to_40</metpo:BactoTrait>
    </owl:Class>
    


    <!-- https://w3id.org/metpo/000177 -->

    <owl:Class rdf:about="https://w3id.org/metpo/000177">
        <rdfs:subClassOf rdf:resource="https://w3id.org/metpo/000013"/>
        <oboInOwl:hasExactSynonym>Thermophile</oboInOwl:hasExactSynonym>
        <rdfs:label>Temperature Range C high (&gt; 40)</rdfs:label>
        <metpo:BactoTrait>TR_&gt;40</metpo:BactoTrait>
    </owl:Class>
    


    <!-- https://w3id.org/metpo/000178 -->

    <owl:Class rdf:about="https://w3id.org/metpo/000178">
        <rdfs:subClassOf rdf:resource="https://w3id.org/metpo/000014"/>
        <oboInOwl:hasExactSynonym>Acid Tolerant</oboInOwl:hasExactSynonym>
        <oboInOwl:hasExactSynonym>Acidophile</oboInOwl:hasExactSynonym>
        <oboInOwl:hasExactSynonym>Extreme Acidophile</oboInOwl:hasExactSynonym>
        <oboInOwl:hasExactSynonym>Facultative acidophile</oboInOwl:hasExactSynonym>
        <oboInOwl:hasExactSynonym>Obligative acidophile</oboInOwl:hasExactSynonym>
        <rdfs:label>pH Optimum low (0 - 6)</rdfs:label>
        <metpo:BactoTrait>pHO_0_to_6</metpo:BactoTrait>
    </owl:Class>
    


    <!-- https://w3id.org/metpo/000179 -->

    <owl:Class rdf:about="https://w3id.org/metpo/000179">
        <rdfs:subClassOf rdf:resource="https://w3id.org/metpo/000014"/>
        <oboInOwl:hasExactSynonym>Alkali Tolerant</oboInOwl:hasExactSynonym>
        <oboInOwl:hasExactSynonym>Neutrophile</oboInOwl:hasExactSynonym>
        <rdfs:label>pH Optimum mid1 (6 - 7)</rdfs:label>
        <metpo:BactoTrait>pHO_6_to_7</metpo:BactoTrait>
    </owl:Class>
    


    <!-- https://w3id.org/metpo/000180 -->

    <owl:Class rdf:about="https://w3id.org/metpo/000180">
        <rdfs:subClassOf rdf:resource="https://w3id.org/metpo/000014"/>
        <oboInOwl:hasExactSynonym>Alkali Tolerant</oboInOwl:hasExactSynonym>
        <oboInOwl:hasExactSynonym>Alkaliphile</oboInOwl:hasExactSynonym>
        <oboInOwl:hasExactSynonym>Neutrophile</oboInOwl:hasExactSynonym>
        <rdfs:label>pH Optimum mid2 (7 - 8)</rdfs:label>
        <metpo:BactoTrait>pHO_7_to_8</metpo:BactoTrait>
    </owl:Class>
    


    <!-- https://w3id.org/metpo/000181 -->

    <owl:Class rdf:about="https://w3id.org/metpo/000181">
        <rdfs:subClassOf rdf:resource="https://w3id.org/metpo/000014"/>
        <oboInOwl:hasExactSynonym>Alkali Tolerant</oboInOwl:hasExactSynonym>
        <oboInOwl:hasExactSynonym>Alkaliphile</oboInOwl:hasExactSynonym>
        <oboInOwl:hasExactSynonym>Extreme Alkaliphile</oboInOwl:hasExactSynonym>
        <rdfs:label>pH Optimum high (8 - 14)</rdfs:label>
        <metpo:BactoTrait>pHO_8_to_14</metpo:BactoTrait>
    </owl:Class>
    


    <!-- https://w3id.org/metpo/000182 -->

    <owl:Class rdf:about="https://w3id.org/metpo/000182">
        <rdfs:subClassOf rdf:resource="https://w3id.org/metpo/000015"/>
        <oboInOwl:hasExactSynonym>Acid Tolerant</oboInOwl:hasExactSynonym>
        <oboInOwl:hasExactSynonym>Acidophile</oboInOwl:hasExactSynonym>
        <oboInOwl:hasExactSynonym>Extreme Acidophile</oboInOwl:hasExactSynonym>
        <oboInOwl:hasExactSynonym>Facultative acidophile</oboInOwl:hasExactSynonym>
        <oboInOwl:hasExactSynonym>Obligative acidophile</oboInOwl:hasExactSynonym>
        <rdfs:label>pH Range very low (0 - 4)</rdfs:label>
        <metpo:BactoTrait>pHR_0_to_4</metpo:BactoTrait>
    </owl:Class>
    


    <!-- https://w3id.org/metpo/000183 -->

    <owl:Class rdf:about="https://w3id.org/metpo/000183">
        <rdfs:subClassOf rdf:resource="https://w3id.org/metpo/000015"/>
        <oboInOwl:hasExactSynonym>Acid Tolerant</oboInOwl:hasExactSynonym>
        <oboInOwl:hasExactSynonym>Acidophile</oboInOwl:hasExactSynonym>
        <oboInOwl:hasExactSynonym>Facultative acidophile</oboInOwl:hasExactSynonym>
        <oboInOwl:hasExactSynonym>Obligative acidophile</oboInOwl:hasExactSynonym>
        <rdfs:label>pH Range low (4 - 6)</rdfs:label>
        <metpo:BactoTrait>pHR_4_to_6</metpo:BactoTrait>
    </owl:Class>
    


    <!-- https://w3id.org/metpo/000184 -->

    <owl:Class rdf:about="https://w3id.org/metpo/000184">
        <rdfs:subClassOf rdf:resource="https://w3id.org/metpo/000015"/>
        <oboInOwl:hasExactSynonym>Alkali Tolerant</oboInOwl:hasExactSynonym>
        <oboInOwl:hasExactSynonym>Facultative acidophile</oboInOwl:hasExactSynonym>
        <oboInOwl:hasExactSynonym>Neutrophile</oboInOwl:hasExactSynonym>
        <rdfs:label>pH Range mid1 (6 - 7)</rdfs:label>
        <metpo:BactoTrait>pHR_6_to_7</metpo:BactoTrait>
    </owl:Class>
    


    <!-- https://w3id.org/metpo/000185 -->

    <owl:Class rdf:about="https://w3id.org/metpo/000185">
        <rdfs:subClassOf rdf:resource="https://w3id.org/metpo/000015"/>
        <oboInOwl:hasExactSynonym>Alkali Tolerant</oboInOwl:hasExactSynonym>
        <oboInOwl:hasExactSynonym>Alkaliphile</oboInOwl:hasExactSynonym>
        <oboInOwl:hasExactSynonym>Facultative acidophile</oboInOwl:hasExactSynonym>
        <oboInOwl:hasExactSynonym>Neutrophile</oboInOwl:hasExactSynonym>
        <rdfs:label>pH Range mid2 (7 - 8)</rdfs:label>
        <metpo:BactoTrait>pHR_7_to_8</metpo:BactoTrait>
    </owl:Class>
    


    <!-- https://w3id.org/metpo/000186 -->

    <owl:Class rdf:about="https://w3id.org/metpo/000186">
        <rdfs:subClassOf rdf:resource="https://w3id.org/metpo/000015"/>
        <oboInOwl:hasExactSynonym>Alkali Tolerant</oboInOwl:hasExactSynonym>
        <oboInOwl:hasExactSynonym>Alkaliphile</oboInOwl:hasExactSynonym>
        <oboInOwl:hasExactSynonym>Extreme Alkaliphile</oboInOwl:hasExactSynonym>
        <oboInOwl:hasExactSynonym>Facultative acidophile</oboInOwl:hasExactSynonym>
        <rdfs:label>pH Range mid3 (8 - 10)</rdfs:label>
        <metpo:BactoTrait>pHR_8_to_10</metpo:BactoTrait>
    </owl:Class>
    


    <!-- https://w3id.org/metpo/000187 -->

    <owl:Class rdf:about="https://w3id.org/metpo/000187">
        <rdfs:subClassOf rdf:resource="https://w3id.org/metpo/000015"/>
        <oboInOwl:hasExactSynonym>Alkali Tolerant</oboInOwl:hasExactSynonym>
        <oboInOwl:hasExactSynonym>Alkaliphile</oboInOwl:hasExactSynonym>
        <oboInOwl:hasExactSynonym>Extreme Alkaliphile</oboInOwl:hasExactSynonym>
        <rdfs:label>pH Range high (10 - 14)</rdfs:label>
        <metpo:BactoTrait>10_to_14</metpo:BactoTrait>
    </owl:Class>
    


    <!-- https://w3id.org/metpo/000188 -->

    <owl:Class rdf:about="https://w3id.org/metpo/000188">
        <rdfs:subClassOf rdf:resource="https://w3id.org/metpo/000016"/>
        <oboInOwl:hasExactSynonym>Halotolerant</oboInOwl:hasExactSynonym>
        <oboInOwl:hasExactSynonym>Non-halophile</oboInOwl:hasExactSynonym>
        <rdfs:label>% NaCl Optimum low (&lt;= 1)</rdfs:label>
        <metpo:BactoTrait>NaR_&lt;=1</metpo:BactoTrait>
    </owl:Class>
    


    <!-- https://w3id.org/metpo/000189 -->

    <owl:Class rdf:about="https://w3id.org/metpo/000189">
        <rdfs:subClassOf rdf:resource="https://w3id.org/metpo/000016"/>
        <oboInOwl:hasExactSynonym>Halotolerant</oboInOwl:hasExactSynonym>
        <oboInOwl:hasExactSynonym>Slight halophile</oboInOwl:hasExactSynonym>
        <rdfs:label>% NaCl Optimum mid1 (1 - 3)</rdfs:label>
        <metpo:BactoTrait>NaR_1_to_3</metpo:BactoTrait>
    </owl:Class>
    


    <!-- https://w3id.org/metpo/000190 -->

    <owl:Class rdf:about="https://w3id.org/metpo/000190">
        <rdfs:subClassOf rdf:resource="https://w3id.org/metpo/000016"/>
        <oboInOwl:hasExactSynonym>Halotolerant</oboInOwl:hasExactSynonym>
        <oboInOwl:hasExactSynonym>Moderate halophile</oboInOwl:hasExactSynonym>
        <rdfs:label>% NaCl Optimum mid2 (3 - 8)</rdfs:label>
        <metpo:BactoTrait>NaR_3_to_8</metpo:BactoTrait>
    </owl:Class>
    


    <!-- https://w3id.org/metpo/000191 -->

    <owl:Class rdf:about="https://w3id.org/metpo/000191">
        <rdfs:subClassOf rdf:resource="https://w3id.org/metpo/000016"/>
        <oboInOwl:hasExactSynonym>Extreme halophile</oboInOwl:hasExactSynonym>
        <rdfs:label>% NaCl Optimum high (&gt; 8)</rdfs:label>
        <metpo:BactoTrait>NaR_&gt;8</metpo:BactoTrait>
    </owl:Class>
    


    <!-- https://w3id.org/metpo/000192 -->

    <owl:Class rdf:about="https://w3id.org/metpo/000192">
        <rdfs:subClassOf rdf:resource="https://w3id.org/metpo/000017"/>
        <oboInOwl:hasExactSynonym>Halotolerant</oboInOwl:hasExactSynonym>
        <oboInOwl:hasExactSynonym>Non-halophile</oboInOwl:hasExactSynonym>
        <rdfs:label>% NaCl Range low (&lt;= 1)</rdfs:label>
        <metpo:BactoTrait>NaO_&lt;=1</metpo:BactoTrait>
    </owl:Class>
    


    <!-- https://w3id.org/metpo/000193 -->

    <owl:Class rdf:about="https://w3id.org/metpo/000193">
        <rdfs:subClassOf rdf:resource="https://w3id.org/metpo/000017"/>
        <oboInOwl:hasExactSynonym>Halotolerant</oboInOwl:hasExactSynonym>
        <oboInOwl:hasExactSynonym>Slight halophile</oboInOwl:hasExactSynonym>
        <rdfs:label>% NaCl Range mid1 (1 - 3)</rdfs:label>
        <metpo:BactoTrait>NaO_1_to_3</metpo:BactoTrait>
    </owl:Class>
    


    <!-- https://w3id.org/metpo/000194 -->

    <owl:Class rdf:about="https://w3id.org/metpo/000194">
        <rdfs:subClassOf rdf:resource="https://w3id.org/metpo/000017"/>
        <oboInOwl:hasExactSynonym>Halotolerant</oboInOwl:hasExactSynonym>
        <oboInOwl:hasExactSynonym>Moderate halophile</oboInOwl:hasExactSynonym>
        <rdfs:label>% NaCl Range mid2 (3 - 8)</rdfs:label>
        <metpo:BactoTrait>NaO_3_to_8</metpo:BactoTrait>
    </owl:Class>
    


    <!-- https://w3id.org/metpo/000195 -->

    <owl:Class rdf:about="https://w3id.org/metpo/000195">
        <rdfs:subClassOf rdf:resource="https://w3id.org/metpo/000017"/>
        <oboInOwl:hasExactSynonym>Extreme halophile</oboInOwl:hasExactSynonym>
        <rdfs:label>% NaCl Range high (&gt; 8)</rdfs:label>
        <metpo:BactoTrait>NaO_&gt;8</metpo:BactoTrait>
    </owl:Class>
    


    <!-- https://w3id.org/metpo/000196 -->

    <owl:Class rdf:about="https://w3id.org/metpo/000196">
        <rdfs:subClassOf rdf:resource="https://w3id.org/metpo/000018"/>
        <rdfs:label>pH delta very low (&lt;= 1)</rdfs:label>
        <metpo:BactoTrait>pHd_&lt;=1</metpo:BactoTrait>
    </owl:Class>
    


    <!-- https://w3id.org/metpo/000197 -->

    <owl:Class rdf:about="https://w3id.org/metpo/000197">
        <rdfs:subClassOf rdf:resource="https://w3id.org/metpo/000018"/>
        <rdfs:label>pH delta low (1 - 2)</rdfs:label>
        <metpo:BactoTrait>pHd_1_2</metpo:BactoTrait>
    </owl:Class>
    


    <!-- https://w3id.org/metpo/000198 -->

    <owl:Class rdf:about="https://w3id.org/metpo/000198">
        <rdfs:subClassOf rdf:resource="https://w3id.org/metpo/000018"/>
        <rdfs:label>pH delta mid1 (2 - 3)</rdfs:label>
        <metpo:BactoTrait>pHd_2_3</metpo:BactoTrait>
    </owl:Class>
    


    <!-- https://w3id.org/metpo/000199 -->

    <owl:Class rdf:about="https://w3id.org/metpo/000199">
        <rdfs:subClassOf rdf:resource="https://w3id.org/metpo/000018"/>
        <rdfs:label>pH delta mid2 (3 - 4)</rdfs:label>
        <metpo:BactoTrait>pHd_3_4</metpo:BactoTrait>
    </owl:Class>
    


    <!-- https://w3id.org/metpo/000200 -->

    <owl:Class rdf:about="https://w3id.org/metpo/000200">
        <rdfs:subClassOf rdf:resource="https://w3id.org/metpo/000018"/>
        <rdfs:label>pH delta mid3 (4 - 5)</rdfs:label>
        <metpo:BactoTrait>pHd_4_5</metpo:BactoTrait>
    </owl:Class>
    


    <!-- https://w3id.org/metpo/000201 -->

    <owl:Class rdf:about="https://w3id.org/metpo/000201">
        <rdfs:subClassOf rdf:resource="https://w3id.org/metpo/000018"/>
        <rdfs:label>pH delta high (5 - 9)</rdfs:label>
        <metpo:BactoTrait>pHd_5_9</metpo:BactoTrait>
    </owl:Class>
    


    <!-- https://w3id.org/metpo/000202 -->

    <owl:Class rdf:about="https://w3id.org/metpo/000202">
        <rdfs:subClassOf rdf:resource="https://w3id.org/metpo/000019"/>
        <rdfs:label>% NaCl delta low (&lt;= 1)</rdfs:label>
        <metpo:BactoTrait>Nad_&lt;=1</metpo:BactoTrait>
    </owl:Class>
    


    <!-- https://w3id.org/metpo/000203 -->

    <owl:Class rdf:about="https://w3id.org/metpo/000203">
        <rdfs:subClassOf rdf:resource="https://w3id.org/metpo/000019"/>
        <rdfs:label>% NaCl delta mid2 (1 - 3)</rdfs:label>
        <metpo:BactoTrait>Nad_1_3</metpo:BactoTrait>
    </owl:Class>
    


    <!-- https://w3id.org/metpo/000204 -->

    <owl:Class rdf:about="https://w3id.org/metpo/000204">
        <rdfs:subClassOf rdf:resource="https://w3id.org/metpo/000019"/>
        <rdfs:label>% NaCl delta mid2 (3 - 8)</rdfs:label>
        <metpo:BactoTrait>Nad_3_8</metpo:BactoTrait>
    </owl:Class>
    


    <!-- https://w3id.org/metpo/000205 -->

    <owl:Class rdf:about="https://w3id.org/metpo/000205">
        <rdfs:subClassOf rdf:resource="https://w3id.org/metpo/000019"/>
        <rdfs:label>% NaCl delta high (&gt;= 8)</rdfs:label>
        <metpo:BactoTrait>Nad_&gt;8</metpo:BactoTrait>
    </owl:Class>
    


    <!-- https://w3id.org/metpo/000206 -->

    <owl:Class rdf:about="https://w3id.org/metpo/000206">
        <rdfs:subClassOf rdf:resource="https://w3id.org/metpo/000020"/>
        <rdfs:label>Temperature C delta very low (1 - 5)</rdfs:label>
        <metpo:BactoTrait>Td_1_5</metpo:BactoTrait>
    </owl:Class>
    


    <!-- https://w3id.org/metpo/000207 -->

    <owl:Class rdf:about="https://w3id.org/metpo/000207">
        <rdfs:subClassOf rdf:resource="https://w3id.org/metpo/000020"/>
        <rdfs:label>Temperature C delta low (5 - 10)</rdfs:label>
        <metpo:BactoTrait>Td_5_10</metpo:BactoTrait>
    </owl:Class>
    


    <!-- https://w3id.org/metpo/000208 -->

    <owl:Class rdf:about="https://w3id.org/metpo/000208">
        <rdfs:subClassOf rdf:resource="https://w3id.org/metpo/000020"/>
        <rdfs:label>Temperature C delta mid1 (10 - 20)</rdfs:label>
        <metpo:BactoTrait>Td_10_20</metpo:BactoTrait>
    </owl:Class>
    


    <!-- https://w3id.org/metpo/000209 -->

    <owl:Class rdf:about="https://w3id.org/metpo/000209">
        <rdfs:subClassOf rdf:resource="https://w3id.org/metpo/000020"/>
        <rdfs:label>Temperature C delta mid2 (20 - 30)</rdfs:label>
        <metpo:BactoTrait>Td_20_30</metpo:BactoTrait>
    </owl:Class>
    


    <!-- https://w3id.org/metpo/000210 -->

    <owl:Class rdf:about="https://w3id.org/metpo/000210">
        <rdfs:subClassOf rdf:resource="https://w3id.org/metpo/000020"/>
        <rdfs:label>Temperature C delta high (&gt;= 30)</rdfs:label>
        <metpo:BactoTrait>Td_&gt;30</metpo:BactoTrait>
    </owl:Class>
    


    <!-- https://w3id.org/metpo/000211 -->

    <owl:Class rdf:about="https://w3id.org/metpo/000211">
        <rdfs:subClassOf rdf:resource="https://w3id.org/metpo/000021"/>
        <obo:IAO_0000115>A rod-shaped cell.</obo:IAO_0000115>
        <rdfs:label>bacillus</rdfs:label>
    </owl:Class>
    


    <!-- https://w3id.org/metpo/000212 -->

    <owl:Class rdf:about="https://w3id.org/metpo/000212">
        <rdfs:subClassOf rdf:resource="https://w3id.org/metpo/000021"/>
        <obo:IAO_0000115>A cell with multiple branches or extensions.</obo:IAO_0000115>
        <rdfs:label>branced</rdfs:label>
    </owl:Class>
    


    <!-- https://w3id.org/metpo/000213 -->

    <owl:Class rdf:about="https://w3id.org/metpo/000213">
        <rdfs:subClassOf rdf:resource="https://w3id.org/metpo/000021"/>
        <obo:IAO_0000115>A short rod-shaped cell, intermediate between bacillus and coccus.</obo:IAO_0000115>
        <rdfs:label>coccobacillus</rdfs:label>
    </owl:Class>
    


    <!-- https://w3id.org/metpo/000214 -->

    <owl:Class rdf:about="https://w3id.org/metpo/000214">
        <rdfs:subClassOf rdf:resource="https://w3id.org/metpo/000021"/>
        <obo:IAO_0000115>A spherical cell.</obo:IAO_0000115>
        <rdfs:label>coccus</rdfs:label>
    </owl:Class>
    


    <!-- https://w3id.org/metpo/000215 -->

    <owl:Class rdf:about="https://w3id.org/metpo/000215">
        <rdfs:subClassOf rdf:resource="https://w3id.org/metpo/000021"/>
        <obo:IAO_0000115>A curved, crescent-shaped cell.</obo:IAO_0000115>
        <rdfs:label>crescent</rdfs:label>
    </owl:Class>
    


    <!-- https://w3id.org/metpo/000216 -->

    <owl:Class rdf:about="https://w3id.org/metpo/000216">
        <rdfs:subClassOf rdf:resource="https://w3id.org/metpo/000021"/>
        <obo:IAO_0000115>A cell with a slight curve or bend.</obo:IAO_0000115>
        <rdfs:label>curved</rdfs:label>
    </owl:Class>
    


    <!-- https://w3id.org/metpo/000217 -->

    <owl:Class rdf:about="https://w3id.org/metpo/000217">
        <rdfs:subClassOf rdf:resource="https://w3id.org/metpo/000021"/>
        <obo:IAO_0000115>A cell with a curved spiral shape.</obo:IAO_0000115>
        <rdfs:label>curved spiral</rdfs:label>
    </owl:Class>
    


    <!-- https://w3id.org/metpo/000218 -->

    <owl:Class rdf:about="https://w3id.org/metpo/000218">
        <rdfs:subClassOf rdf:resource="https://w3id.org/metpo/000021"/>
        <obo:IAO_0000115>Two spherical cells attached to each other.</obo:IAO_0000115>
        <rdfs:label>diplococcus</rdfs:label>
    </owl:Class>
    


    <!-- https://w3id.org/metpo/000219 -->

    <owl:Class rdf:about="https://w3id.org/metpo/000219">
        <rdfs:subClassOf rdf:resource="https://w3id.org/metpo/000021"/>
        <obo:IAO_0000115>A flat, circular-shaped cell.</obo:IAO_0000115>
        <rdfs:label>disc</rdfs:label>
    </owl:Class>
    


    <!-- https://w3id.org/metpo/000220 -->

    <owl:Class rdf:about="https://w3id.org/metpo/000220">
        <rdfs:subClassOf rdf:resource="https://w3id.org/metpo/000021"/>
        <obo:IAO_0000115>A cell shaped like two spheres connected by a narrow bridge.</obo:IAO_0000115>
        <rdfs:label>dumbbell</rdfs:label>
    </owl:Class>
    


    <!-- https://w3id.org/metpo/000221 -->

    <owl:Class rdf:about="https://w3id.org/metpo/000221">
        <rdfs:subClassOf rdf:resource="https://w3id.org/metpo/000021"/>
        <obo:IAO_0000115>A cell with an elongated oval shape.</obo:IAO_0000115>
        <rdfs:label>ellipsoidal</rdfs:label>
    </owl:Class>
    


    <!-- https://w3id.org/metpo/000222 -->

    <owl:Class rdf:about="https://w3id.org/metpo/000222">
        <rdfs:subClassOf rdf:resource="https://w3id.org/metpo/000021"/>
        <obo:IAO_0000115>A long, thin, thread-like cell.</obo:IAO_0000115>
        <rdfs:label>filament</rdfs:label>
    </owl:Class>
    


    <!-- https://w3id.org/metpo/000223 -->

    <owl:Class rdf:about="https://w3id.org/metpo/000223">
        <rdfs:subClassOf rdf:resource="https://w3id.org/metpo/000021"/>
        <obo:IAO_0000115>A cell shaped like a laboratory flask.</obo:IAO_0000115>
        <rdfs:label>flask</rdfs:label>
    </owl:Class>
    


    <!-- https://w3id.org/metpo/000224 -->

    <owl:Class rdf:about="https://w3id.org/metpo/000224">
        <rdfs:subClassOf rdf:resource="https://w3id.org/metpo/000021"/>
        <obo:IAO_0000115>A cell with a spindle-like shape, wider in the middle and tapering at both ends.</obo:IAO_0000115>
        <rdfs:label>fusiform</rdfs:label>
    </owl:Class>
    


    <!-- https://w3id.org/metpo/000225 -->

    <owl:Class rdf:about="https://w3id.org/metpo/000225">
        <rdfs:subClassOf rdf:resource="https://w3id.org/metpo/000021"/>
        <obo:IAO_0000115>A cell with a spiral shape, forming a three-dimensional helix.</obo:IAO_0000115>
        <rdfs:label>helical</rdfs:label>
    </owl:Class>
    


    <!-- https://w3id.org/metpo/000226 -->

    <owl:Class rdf:about="https://w3id.org/metpo/000226">
        <rdfs:subClassOf rdf:resource="https://w3id.org/metpo/000021"/>
        <obo:IAO_0000115>A cell with an inconsistent or non-uniform shape.</obo:IAO_0000115>
        <rdfs:label>irregular</rdfs:label>
    </owl:Class>
    


    <!-- https://w3id.org/metpo/000227 -->

    <owl:Class rdf:about="https://w3id.org/metpo/000227">
        <rdfs:subClassOf rdf:resource="https://w3id.org/metpo/000021"/>
        <obo:IAO_0000115>A cell with an egg-shaped outline.</obo:IAO_0000115>
        <rdfs:label>oval</rdfs:label>
    </owl:Class>
    


    <!-- https://w3id.org/metpo/000228 -->

    <owl:Class rdf:about="https://w3id.org/metpo/000228">
        <rdfs:subClassOf rdf:resource="https://w3id.org/metpo/000021"/>
        <obo:IAO_0000115>A cell with an egg-like shape, slightly elongated.</obo:IAO_0000115>
        <rdfs:label>ovoid</rdfs:label>
    </owl:Class>
    


    <!-- https://w3id.org/metpo/000229 -->

    <owl:Class rdf:about="https://w3id.org/metpo/000229">
        <rdfs:subClassOf rdf:resource="https://w3id.org/metpo/000021"/>
        <obo:IAO_0000115>A cell capable of assuming various shapes.</obo:IAO_0000115>
        <rdfs:label>pleomorphic</rdfs:label>
    </owl:Class>
    


    <!-- https://w3id.org/metpo/000230 -->

    <owl:Class rdf:about="https://w3id.org/metpo/000230">
        <rdfs:subClassOf rdf:resource="https://w3id.org/metpo/000021"/>
        <obo:IAO_0000115>A cell shaped like a circular band or loop.</obo:IAO_0000115>
        <rdfs:label>ring</rdfs:label>
    </owl:Class>
    


    <!-- https://w3id.org/metpo/000231 -->

    <owl:Class rdf:about="https://w3id.org/metpo/000231">
        <rdfs:subClassOf rdf:resource="https://w3id.org/metpo/000021"/>
        <obo:IAO_0000115>A straight, elongated cell.</obo:IAO_0000115>
        <rdfs:label>rod</rdfs:label>
    </owl:Class>
    


    <!-- https://w3id.org/metpo/000232 -->

    <owl:Class rdf:about="https://w3id.org/metpo/000232">
        <rdfs:subClassOf rdf:resource="https://w3id.org/metpo/000021"/>
        <obo:IAO_0000115>A perfectly round cell.</obo:IAO_0000115>
        <rdfs:label>sphere</rdfs:label>
    </owl:Class>
    


    <!-- https://w3id.org/metpo/000233 -->

    <owl:Class rdf:about="https://w3id.org/metpo/000233">
        <rdfs:subClassOf rdf:resource="https://w3id.org/metpo/000021"/>
        <obo:IAO_0000115>A cell with a shape that tapers at both ends.</obo:IAO_0000115>
        <rdfs:label>spindle</rdfs:label>
    </owl:Class>
    


    <!-- https://w3id.org/metpo/000234 -->

    <owl:Class rdf:about="https://w3id.org/metpo/000234">
        <rdfs:subClassOf rdf:resource="https://w3id.org/metpo/000021"/>
        <obo:IAO_0000115>A cell with a tight, coiled shape.</obo:IAO_0000115>
        <rdfs:label>spiral</rdfs:label>
    </owl:Class>
    


    <!-- https://w3id.org/metpo/000235 -->

    <owl:Class rdf:about="https://w3id.org/metpo/000235">
        <rdfs:subClassOf rdf:resource="https://w3id.org/metpo/000021"/>
        <obo:IAO_0000115>A cell with a long, thin, flexible spiral shape.</obo:IAO_0000115>
        <rdfs:label>spirochete</rdfs:label>
    </owl:Class>
    


    <!-- https://w3id.org/metpo/000236 -->

    <owl:Class rdf:about="https://w3id.org/metpo/000236">
        <rdfs:subClassOf rdf:resource="https://w3id.org/metpo/000021"/>
        <obo:IAO_0000115>A dormant, resistant form of a cell.</obo:IAO_0000115>
        <rdfs:label>spore</rdfs:label>
    </owl:Class>
    


    <!-- https://w3id.org/metpo/000237 -->

    <owl:Class rdf:about="https://w3id.org/metpo/000237">
        <rdfs:subClassOf rdf:resource="https://w3id.org/metpo/000021"/>
        <obo:IAO_0000115>A cell with a cube-like shape.</obo:IAO_0000115>
        <rdfs:label>square</rdfs:label>
    </owl:Class>
    


    <!-- https://w3id.org/metpo/000238 -->

    <owl:Class rdf:about="https://w3id.org/metpo/000238">
        <rdfs:subClassOf rdf:resource="https://w3id.org/metpo/000021"/>
        <obo:IAO_0000115>A cell with multiple pointed projections, resembling a star.</obo:IAO_0000115>
        <rdfs:label>star</rdfs:label>
    </owl:Class>
    


    <!-- https://w3id.org/metpo/000239 -->

    <owl:Class rdf:about="https://w3id.org/metpo/000239">
        <rdfs:subClassOf rdf:resource="https://w3id.org/metpo/000021"/>
        <obo:IAO_0000115>A cell that can assume star-shaped, dumbbell-shaped, or various other forms.</obo:IAO_0000115>
        <rdfs:label>star - dumbbell - pleomorphic</rdfs:label>
    </owl:Class>
    


    <!-- https://w3id.org/metpo/000240 -->

    <owl:Class rdf:about="https://w3id.org/metpo/000240">
        <rdfs:subClassOf rdf:resource="https://w3id.org/metpo/000021"/>
        <obo:IAO_0000115>A cell with a main body and a tail-like extension.</obo:IAO_0000115>
        <rdfs:label>tailed</rdfs:label>
    </owl:Class>
    


    <!-- https://w3id.org/metpo/000241 -->

    <owl:Class rdf:about="https://w3id.org/metpo/000241">
        <rdfs:subClassOf rdf:resource="https://w3id.org/metpo/000021"/>
        <obo:IAO_0000115>A cell with a three-sided shape.</obo:IAO_0000115>
        <rdfs:label>triangular</rdfs:label>
    </owl:Class>
    


    <!-- https://w3id.org/metpo/000242 -->

    <owl:Class rdf:about="https://w3id.org/metpo/000242">
        <rdfs:subClassOf rdf:resource="https://w3id.org/metpo/000021"/>
        <obo:IAO_0000115>A curved rod-shaped cell, resembling a comma.</obo:IAO_0000115>
        <rdfs:label>vibrio</rdfs:label>
    </owl:Class>
    


    <!-- https://w3id.org/metpo/000243 -->

    <owl:Class rdf:about="https://w3id.org/metpo/000243">
        <obo:IAO_0000115>A measurable property of the external environment that influences microbial growth or behavior.</obo:IAO_0000115>
        <rdfs:label>Environmental Parameter</rdfs:label>
    </owl:Class>
    


    <!-- https://w3id.org/metpo/000244 -->

    <owl:Class rdf:about="https://w3id.org/metpo/000244">
        <obo:IAO_0000115>A specific combination of environmental factors under which a microorganism can maintain its lifecycle.</obo:IAO_0000115>
        <rdfs:label>Growth Condition</rdfs:label>
    </owl:Class>
    


    <!-- https://w3id.org/metpo/000245 -->

    <owl:Class rdf:about="https://w3id.org/metpo/000245">
        <obo:IAO_0000115>An inherent characteristic of an organism related to its biological functioning and metabolic processes.</obo:IAO_0000115>
        <rdfs:label>Physiological Trait</rdfs:label>
    </owl:Class>
    


    <!-- https://w3id.org/metpo/000246 -->

    <owl:Class rdf:about="https://w3id.org/metpo/000246">
        <obo:IAO_0000115>A categorization of an organism based on its specific patterns of energy acquisition and material transformation.</obo:IAO_0000115>
        <rdfs:label>Metabolic Classification</rdfs:label>
    </owl:Class>
    


    <!-- https://w3id.org/metpo/000247 -->

    <owl:Class rdf:about="https://w3id.org/metpo/000247">
        <obo:IAO_0000115>A distinctive property of a cell that contributes to its structure, function, or behavior.</obo:IAO_0000115>
        <rdfs:label>Cellular Characteristic</rdfs:label>
    </owl:Class>
    


    <!-- https://w3id.org/metpo/000248 -->

    <owl:Class rdf:about="https://w3id.org/metpo/000248">
        <obo:IAO_0000115>A morphological, genetic, or physiological characteristic used for classifying organisms within a systematic hierarchy.</obo:IAO_0000115>
        <rdfs:label>Taxonomic Feature</rdfs:label>
    </owl:Class>
    


    <!-- https://w3id.org/metpo/000249 -->

    <owl:Class rdf:about="https://w3id.org/metpo/000249">
        <obo:IAO_0000115>A heritable change in structure, function, or behavior that increases a microorganism&apos;s fitness in a specific environment.</obo:IAO_0000115>
        <rdfs:label>Microbial Adaptation</rdfs:label>
    </owl:Class>
    


    <!-- https://w3id.org/metpo/000250 -->

    <owl:Class rdf:about="https://w3id.org/metpo/000250">
        <obo:IAO_0000115>A quantifiable factor that affects or describes the rate or extent of microbial population increase.</obo:IAO_0000115>
        <rdfs:label>Growth Parameter</rdfs:label>
    </owl:Class>
    


    <!-- https://w3id.org/metpo/000251 -->

    <owl:Class rdf:about="https://w3id.org/metpo/000251">
        <obo:IAO_0000115>A physical component or arrangement of components that contributes to an organism&apos;s form or architecture.</obo:IAO_0000115>
        <rdfs:label>Structural Feature</rdfs:label>
    </owl:Class>
    


    <!-- https://w3id.org/metpo/000252 -->

    <owl:Class rdf:about="https://w3id.org/metpo/000252">
        <obo:IAO_0000115>A physiological adjustment that enables an organism to survive and reproduce at a specific temperature range.</obo:IAO_0000115>
        <rdfs:label>Temperature Adaptation</rdfs:label>
    </owl:Class>
    


    <!-- https://w3id.org/metpo/000253 -->

    <owl:Class rdf:about="https://w3id.org/metpo/000253">
        <obo:IAO_0000115>A set of mechanisms that allows an organism to maintain homeostasis in environments with particular salt concentrations.</obo:IAO_0000115>
        <rdfs:label>Salinity Adaptation</rdfs:label>
    </owl:Class>
    


    <!-- https://w3id.org/metpo/000254 -->

    <owl:Class rdf:about="https://w3id.org/metpo/000254">
        <obo:IAO_0000115>A combination of cellular processes that permits survival and growth under specific hydrogen ion concentrations.</obo:IAO_0000115>
        <rdfs:label>pH Adaptation</rdfs:label>
    </owl:Class>
    


    <!-- https://w3id.org/metpo/000255 -->

    <owl:Class rdf:about="https://w3id.org/metpo/000255">
        <obo:IAO_0000115>The specific need for or tolerance of molecular oxygen that characterizes an organism&apos;s metabolic processes.</obo:IAO_0000115>
        <rdfs:label>Oxygen Requirement</rdfs:label>
    </owl:Class>
    


    <!-- https://w3id.org/metpo/000256 -->

    <owl:Class rdf:about="https://w3id.org/metpo/000256">
        <obo:IAO_0000115>The ability to assimilate and metabolize specific carbon-containing compounds for cellular growth and maintenance.</obo:IAO_0000115>
        <rdfs:label>Carbon Source Utilization</rdfs:label>
    </owl:Class>
    


    <!-- https://w3id.org/metpo/000257 -->

    <owl:Class rdf:about="https://w3id.org/metpo/000257">
        <obo:IAO_0000115>The mechanism by which an organism obtains energy for cellular activities and biosynthesis.</obo:IAO_0000115>
        <rdfs:label>Energy Acquisition Mode</rdfs:label>
    </owl:Class>
    


    <!-- https://w3id.org/metpo/000258 -->

    <owl:Class rdf:about="https://w3id.org/metpo/000258">
        <obo:IAO_0000115>The class of compounds or elements from which an organism extracts electrons for energy-generating reactions.</obo:IAO_0000115>
        <rdfs:label>Electron Donor Type</rdfs:label>
    </owl:Class>
    


    <!-- https://w3id.org/metpo/000259 -->

    <owl:Class rdf:about="https://w3id.org/metpo/000259">
        <obo:IAO_0000115>The biochemical and mechanical processes that enable an organism to move through its environment.</obo:IAO_0000115>
        <rdfs:label>Motility Mechanism</rdfs:label>
    </owl:Class>
    


    <!-- https://w3id.org/metpo/000260 -->

    <owl:Class rdf:about="https://w3id.org/metpo/000260">
        <obo:IAO_0000115>A specialized cellular component that generates force or facilitates movement in microorganisms.</obo:IAO_0000115>
        <rdfs:label>Motility Structure</rdfs:label>
    </owl:Class>
    


    <!-- https://w3id.org/metpo/000261 -->

    <owl:Class rdf:about="https://w3id.org/metpo/000261">
        <obo:IAO_0000115>A classification of resistant dormant structures produced by bacteria based on their formation and properties.</obo:IAO_0000115>
        <rdfs:label>Bacterial Spore Type</rdfs:label>
    </owl:Class>
    


    <!-- https://w3id.org/metpo/000262 -->

    <owl:Class rdf:about="https://w3id.org/metpo/000262">
        <obo:IAO_0000115>A distinct category of reproductive or survival structures produced by fungi, characterized by specific morphology and function.</obo:IAO_0000115>
        <rdfs:label>Fungal Spore Type</rdfs:label>
    </owl:Class>
    


    <!-- https://w3id.org/metpo/000263 -->

    <owl:Class rdf:about="https://w3id.org/metpo/000263">
        <obo:IAO_0000115>A specialized cellular formation that functions in the propagation of genetic material to produce new individuals.</obo:IAO_0000115>
        <rdfs:label>Reproductive Structure</rdfs:label>
    </owl:Class>
    


    <!-- https://w3id.org/metpo/000264 -->

    <owl:Class rdf:about="https://w3id.org/metpo/000264">
        <obo:IAO_0000115>A specialized cellular state or formation that enables survival during adverse environmental conditions with reduced metabolic activity.</obo:IAO_0000115>
        <rdfs:label>Dormancy Structure</rdfs:label>
    </owl:Class>
    


    <!-- https://w3id.org/metpo/000265 -->

    <owl:Class rdf:about="https://w3id.org/metpo/000265">
        <obo:IAO_0000115>A set of physiological and molecular mechanisms that enable survival under specific hydrostatic pressure conditions.</obo:IAO_0000115>
        <rdfs:label>Pressure Adaptation Type</rdfs:label>
    </owl:Class>
    


    <!-- https://w3id.org/metpo/000266 -->

    <owl:Class rdf:about="https://w3id.org/metpo/000266">
        <obo:IAO_0000115>The span of hydrostatic pressures within which an organism can maintain viability and cellular functions.</obo:IAO_0000115>
        <rdfs:label>Pressure Tolerance Range</rdfs:label>
    </owl:Class>
    


    <!-- https://w3id.org/metpo/000267 -->

    <owl:Class rdf:about="https://w3id.org/metpo/000267">
        <obo:IAO_0000115>A distinctive characteristic of an organism&apos;s genetic material related to its sequence, structure, or organization.</obo:IAO_0000115>
        <rdfs:label>GenomicFeature</rdfs:label>
    </owl:Class>
    


    <!-- https://w3id.org/metpo/000268 -->

    <owl:Class rdf:about="https://w3id.org/metpo/000268">
        <obo:IAO_0000115>A measurable spatial attribute of a cell that describes its size in one or more directions.</obo:IAO_0000115>
        <rdfs:label>Cell Dimension</rdfs:label>
    </owl:Class>
    


    <!-- https://w3id.org/metpo/000269 -->

    <owl:Class rdf:about="https://w3id.org/metpo/000269">
        <obo:IAO_0000115>The specific environmental condition at which an organism achieves its maximum growth rate or metabolic efficiency.</obo:IAO_0000115>
        <rdfs:label>Optimal Growth Parameter</rdfs:label>
    </owl:Class>
    


    <!-- https://w3id.org/metpo/000270 -->

    <owl:Class rdf:about="https://w3id.org/metpo/000270">
        <obo:IAO_0000115>The span of environmental conditions within which an organism can sustain growth and reproduction.</obo:IAO_0000115>
        <rdfs:label>Growth Range Parameter</rdfs:label>
    </owl:Class>
    


    <!-- https://w3id.org/metpo/000271 -->

    <owl:Class rdf:about="https://w3id.org/metpo/000271">
        <obo:IAO_0000115>A quantitative measure of an organism&apos;s ability to withstand variations in a specific environmental factor.</obo:IAO_0000115>
        <rdfs:label>Growth Tolerance Metric</rdfs:label>
    </owl:Class>
    


    <!-- https://w3id.org/metpo/000272 -->

    <owl:Class rdf:about="https://w3id.org/metpo/000272">
        <obo:IAO_0000115>The three-dimensional geometric form of a microbial cell as determined by its cell wall and cytoskeletal structures.</obo:IAO_0000115>
        <rdfs:label>Cell Shape</rdfs:label>
    </owl:Class>
    


    <!-- https://w3id.org/metpo/000273 -->

    <owl:Class rdf:about="https://w3id.org/metpo/000273">
        <obo:IAO_0000115>The spatial organization of multiple cells in relation to each other following cell division.</obo:IAO_0000115>
        <rdfs:label>Cell Arrangement</rdfs:label>
    </owl:Class>
    


    <!-- https://w3id.org/metpo/000274 -->

    <owl:Class rdf:about="https://w3id.org/metpo/000274">
        <obo:IAO_0000115>The macroscopic appearance and structure of a population of microorganisms growing on a solid medium.</obo:IAO_0000115>
        <rdfs:label>Colony Morphology</rdfs:label>
    </owl:Class>
</rdf:RDF>



<!-- Generated by the OWL API (version 4.5.29) https://github.com/owlcs/owlapi -->

